theories/L6_PCPS/Heap/heap_defs.v
@@ -9,6 +9,7 @@ From ExtLib Require Import Structures.Monad Data.Monads.OptionMonad Core.Type.
 From L6 Require Import cps cps_util eval List_util Ensembles_util functions
         identifiers Heap.heap tactics.
 Require Import compcert.lib.Coqlib.
+Import ListNotations.
 
 
 Open Scope Ensembles_scope.
@@ -19,9 +20,8 @@ Module HeapDefs (H : Heap).
 
   (** * Heap definitions *)
 
-  (** A value is a location plus or a location paired with a function pointer offset *)
+  (** A value is a location or a function pointer offset *)
   Inductive value : Type :=
-  (* Just a location. Either a data pointer of a function pointer *)
   | Loc : loc -> value
   | FunPtr : fundefs -> var -> value.
 
@@ -44,302 +44,6 @@ Module HeapDefs (H : Heap).
   | OOT : ans (* out of time *)
   | OOM : ans (* out of memory. XXX not used *).
   
-  (** Syntactic approximation of results with fuel *)
-  Fixpoint res_approx_fuel (n : nat) (r1 r2 : res) : Prop :=
-    let '(v1, H1) := r1 in
-    let '(v2, H2) := r2 in
-    match v1, v2 with
-      | Loc l1, Loc l2 => 
-        match get l1 H1 with
-          | Some (Constr c vs1) =>
-            exists vs2, 
-              get l2 H2 = Some (Constr c vs2) /\
-              forall i, (i < n)%nat ->
-                   match n with
-                     | 0%nat => True
-                     | S n' =>
-                       Forall2
-                         (fun l1 l2 => res_approx_fuel (n'-(n'-i)) (l1, H1) (l2, H2)) vs1 vs2
-                   end
-          | Some (Env rho1) =>
-            exists rho2,
-              get l2 H2 = Some (Env rho2) /\
-              (forall x,  (exists v1 v2, M.get x rho1 = Some v1 /\
-                               M.get x rho2 = Some v2 /\
-                               (forall i, (i < n)%nat ->
-                                     match n with
-                                       | 0%nat => True
-                                       | S n' => res_approx_fuel (n'-(n'-i)) (v1, H1) (v2, H2)
-                                     end)) \/
-                     (M.get x rho1 = None /\ M.get x rho2 = None))
-          | None => True
-        end
-      | FunPtr B1 f1, FunPtr B2 f2 => f1 = f2 /\ B1 = B2
-      | _, _ => False
-    end.
-  
-  (** Result equivalence. Two results represent the exact same value *)
-  Definition res_equiv (r1 r2 : res) : Prop :=
-    forall n, res_approx_fuel n r1 r2 /\ res_approx_fuel n r2 r1.
-  
-  Infix "≈" := res_equiv (at level 70, no associativity).
-  
-  Definition ans_equiv (a1 a2 : ans) :=
-    match a1, a2 with
-      | Res r1, Res r2 => r1 ≈ r2
-      | OOT, OOT => True
-      | _, _  => False
-    end.
-  
-  (** Approximation lifted to the environments *)
-  Definition heap_env_approx (S : Ensemble var) p1 p2 : Prop :=
-    let '(H1, rho1) := p1 in
-    let '(H2, rho2) := p2 in
-    forall x l, x \in S ->
-           M.get x rho1 = Some l ->
-           exists l', M.get x rho2 = Some l' /\
-                 (l, H1) ≈ (l', H2).
-  
-  (** Equivalence lifted to the environments *)
-  Definition heap_env_equiv S p1 p2 : Prop :=
-    heap_env_approx S p1 p2 /\
-    heap_env_approx S p2 p1.
-  
-  Notation "S |- p1 ⩪ p2" := (heap_env_equiv S p1 p2)
-                               (at level 70, no associativity).
-  
-  Definition block_equiv (p1 p2 : heap block * block) :=
-    let '(H1, b1) := p1 in
-    let '(H2, b2) := p2 in
-    match b1, b2 with
-      | Constr c1 vs1, Constr c2 vs2 =>
-        c1 = c2 /\ Forall2 (fun v1 v2 => (v1, H1) ≈ (v2, H2)) vs1 vs2
-      | Env rho1, Env rho2 => Full_set _ |- (H1, rho1) ⩪ (H2, rho2)
-      | _, _ => False
-    end.
-  
-  Definition heap_approx (S : Ensemble loc) H1 H2 : Prop :=
-    forall b1 l, l \in S -> get l H1 = Some b1 ->
-           exists b2, get l H2 = Some b2 /\ block_equiv (H1, b1) (H2, b2).
-  
-  Definition heap_equiv (S : Ensemble loc) H1 H2 : Prop :=
-    heap_approx S H1 H2 /\ heap_approx S H2 H1. 
-
-  Notation  "S |- H1 ≃ H2" := (heap_equiv S H1 H2)
-                                (at level 70, no associativity).
-  
-  (** Equivalent definition, unfolding the recursion *)
-  Definition res_approx_fuel' (n : nat) (r1 r2 : res) : Prop :=
-    let '(v1, H1) := r1 in
-    let '(v2, H2) := r2 in
-    match v1, v2 with
-      | Loc l1, Loc l2 => 
-        match get l1 H1 with
-          | Some (Constr c vs1) =>
-            exists vs2, 
-              get l2 H2 = Some (Constr c vs2) /\
-              forall i, (i < n)%nat ->
-                   Forall2 (fun l1 l2 => res_approx_fuel i (l1, H1) (l2, H2)) vs1 vs2
-          | Some (Env rho1) =>
-            exists rho2,
-              get l2 H2 = Some (Env rho2) /\
-               (forall x, (exists v1 v2, M.get x rho1 = Some v1 /\
-                               M.get x rho2 = Some v2 /\
-                               (forall i, (i < n)%nat ->
-                                     res_approx_fuel i (v1, H1) (v2, H2))) \/
-                     (M.get x rho1 = None /\ M.get x rho2 = None))
-          | None => True
-        end
-      | FunPtr B1 f1, FunPtr B2 f2 => f1 = f2 /\ B1 = B2
-      | _, _ => False
-    end.
-  
-  (** Equivalence of the two definitions *)
-  Lemma res_approx_fuel_eq n r1 r2 :
-    res_approx_fuel n r1 r2 <-> res_approx_fuel' n r1 r2.
-  Proof.
-    destruct n; destruct r1 as [[l1 | B1 f1] H1]; destruct r2 as [[l2 | B2 f2] H2]; simpl.
-    - destruct (get l1 H1) as [[c1 vs1 | rho1]|]; [| | now firstorder ].
-      + split.
-        * intros [vs [H _ ]]. eexists. split; eauto.
-          intros; omega.
-        * intros [vs [H _ ]]. eexists. split; eauto.
-      + split.
-        * intros [vs [H Hb ]]. eexists. split; eauto.
-          intros x. destruct (Hb x) as [Hb1 | Hb1]; eauto. 
-          destruct Hb1 as [v1 [v2 [Hget1 [Hget2 Ht]]]].
-          left. repeat eexists; eauto. intros; omega.
-        * intros [vs [H Hb ]]. eexists. split; eauto.
-          intros x. destruct (Hb x) as [Hb1 | Hb1]; eauto. 
-          destruct Hb1 as [v1 [v2 [Hget1 [Hget2 Ht]]]].
-          left. repeat eexists; eauto.
-    - split; eauto.
-    - split; eauto.   
-    - now firstorder.
-    - destruct (get l1 H1) as [[c1 vs1 | rho1 ]|]; [| | now firstorder ].
-      + split.
-        * intros [vs [H Hi]]. eexists. split; eauto.
-          intros i Hlt.
-          assert (Heq : (i =  n - (n - i))%nat) by omega. rewrite Heq.
-          eauto.
-        * intros [vs [H Hin]]. eexists. split; eauto.
-          intros i Hlt.
-          assert (Heq : (i =  n - (n - i))%nat) by omega. rewrite <- Heq.
-          eauto.
-      + split.
-        * intros [vs [H Hb ]]. eexists. split; eauto.
-          intros x. destruct (Hb x) as [Hb1 | Hb1]; eauto. 
-          destruct Hb1 as [v1 [v2 [Hget1 [Hget2 Ht]]]].
-          left. repeat eexists; eauto.
-          intros i Hlt.
-          assert (Heq : (i =  n - (n - i))%nat) by omega. rewrite Heq.
-          eauto.
-        * intros [vs [H Hb ]]. eexists. split; eauto.
-          intros x. destruct (Hb x) as [Hb1 | Hb1]; eauto. 
-          destruct Hb1 as [v1 [v2 [Hget1 [Hget2 Ht]]]].
-          left. repeat eexists; eauto.
-          intros i Hlt.
-          assert (Heq : (i =  n - (n - i))%nat) by omega. rewrite <- Heq.
-          eauto.
-    - split; eauto.
-    - split; eauto.   
-    - now firstorder.
-  Qed.
-
-  Opaque res_approx_fuel.
-  
- (** Equivalent definition for [res_equiv] *)
-  Definition res_equiv' (r1 r2 : res) : Prop :=
-    let '(v1, H1) := r1 in
-    let '(v2, H2) := r2 in
-    match v1, v2 with
-      | Loc l1, Loc l2 =>
-        match get l1 H1, get l2 H2 with
-          | Some b1, Some b2 => block_equiv (H1, b1) (H2, b2)
-          | None, None => True
-          | _, _ => False
-        end
-      | FunPtr B1 f1, FunPtr B2 f2 =>
-        B1 = B2 /\ f1 = f2
-      | _, _ => False
-    end.
-
-  (* TODO move *)
-  Lemma Forall2_flip {A B} (R :  A -> B -> Prop) (l1 : list A) (l2 : list B) :
-    Forall2 (fun x y => R x y) l1 l2 ->
-    Forall2 (fun x y => R y x) l2 l1.
-  Proof.
-    intros H1. induction H1; eauto.
-  Qed.
-  
-  Lemma res_equiv_eq r1 r2 :
-    res_equiv r1 r2 <-> res_equiv' r1 r2.
-  Proof.
-    destruct r1 as [[l1 | B1 f1] H1]; destruct r2 as [[l2 | B2 f2] H2]; simpl.
-    unfold res_equiv. split. 
-    - intros H. assert (H0 := H 0%nat).
-      destruct H0 as [Hal Har]. rewrite !res_approx_fuel_eq in Hal, Har.
-      simpl in *. destruct (get l1 H1) as [ v |] eqn:Hget1.
-      + destruct v as [c1 vs1 | rho1 B1 off1 ].
-        * destruct Hal as [vs2 [Hget2 Hi]].
-          rewrite Hget2 in Har.
-          destruct Har as [vs1' [Hget1' Hi']]. inv Hget1'. 
-          rewrite Hget2. split; eauto.
-          eapply Forall2_forall. constructor. exact 0%nat.
-          intros n. specialize (H (S n)). rewrite !res_approx_fuel_eq in H. 
-          edestruct H as [Hal' Har']. simpl in Hal', Har'.
-          rewrite Hget1 in Hal'. rewrite Hget2 in Har'. 
-          destruct Hal' as [vs2' [Hget2' Hi2]]. subst_exp.
-          destruct Har' as [vs1 [Hget1' Hi1]]. subst_exp.
-          eapply Forall2_conj.
-          eapply Hi2. omega.
-          eapply Forall2_flip. eapply Hi1. omega.
-        * destruct Hal as [rho2 [Hget2 Hi1]].
-          rewrite Hget2 in Har.
-          destruct Har as [rho1' [Hget1' Hi2]]. inv Hget1'. 
-          rewrite Hget2. split; eauto; intros x l _ Hget.
-          { destruct (Hi1 x) as [[v1 [v2 [Hgetv1 [Hgetv2 Hi]]]] | [Hn1 Hn2]]; try congruence.
-            subst_exp. eexists; split; eauto.
-            intros n.
-            specialize (H (S n)). rewrite !res_approx_fuel_eq in H. 
-            edestruct H as [Hal' Har']. simpl in Hal', Har'.
-            rewrite Hget1 in Hal'. rewrite Hget2 in Har'. 
-            destruct Hal' as [rho2' [Hget2' Hin2]]. subst_exp.
-            destruct Har' as [rho1 [Hget1' Hin1]]. subst_exp.
-            destruct (Hin1 x) as [[v1' [v2' [Hgetv1' [Hgetv2' Hi1']]]] | [Hn1 Hn2]]; try congruence.
-            repeat subst_exp.
-            destruct (Hin2 x) as [[v1'' [v2'' [Hgetv1' [Hgetv2' Hi2']]]] | [Hn1 Hn2]]; try congruence.
-            repeat subst_exp. split; eauto. }
-          { destruct (Hi1 x) as [[v1 [v2 [Hgetv1 [Hgetv2 Hi]]]] | [Hn1 Hn2]]; try congruence.
-            subst_exp. eexists; split; eauto.
-            intros n.
-            specialize (H (S n)). rewrite !res_approx_fuel_eq in H. 
-            edestruct H as [Hal' Har']. simpl in Hal', Har'.
-            rewrite Hget1 in Hal'. rewrite Hget2 in Har'. 
-            destruct Hal' as [rho2' [Hget2' Hin2]]. subst_exp.
-            destruct Har' as [rho1 [Hget1' Hin1]]. subst_exp.
-            destruct (Hin1 x) as [[v1' [v2' [Hgetv1' [Hgetv2' Hi1']]]] | [Hn1 Hn2]]; try congruence.
-            repeat subst_exp.
-            destruct (Hin2 x) as [[v1'' [v2'' [Hgetv1' [Hgetv2' Hi2']]]] | [Hn1 Hn2]]; try congruence.          
-            repeat subst_exp. split; eauto. }
-      + destruct (get l2 H2); eauto.
-        destruct b.
-        destruct Har as [vs2 [Heq _]]; discriminate.
-        destruct Har as [vs2 [Heq _]]; discriminate.
-    - destruct (get l1 H1) eqn:Hget1.
-      + destruct b as [ c vs1 | rho1 B1 off1 ].
-        * destruct (get l2 H2) eqn:Hget2; try contradiction.
-          destruct b as [c' vs2 |]; try contradiction.
-          intros [Heq Hall] n. subst. rewrite !res_approx_fuel_eq.
-          simpl. rewrite Hget1, Hget2. split.
-          
-          eexists. split. reflexivity.
-          intros. eapply Forall2_monotonic; [| eassumption ].
-          now intros v1 v2 [Hl Hr]; eauto. 
-
-          eexists. split. reflexivity.
-          intros. eapply Forall2_flip. eapply Forall2_monotonic; [| eassumption ].
-          now intros v1 v2 [Hl Hr]; eauto. 
-        * destruct (get l2 H2) eqn:Hget2; try contradiction.
-          destruct b as [ | rho2]; try contradiction.
-          intros [Hl Hr] n. rewrite !res_approx_fuel_eq.
-          simpl. rewrite Hget1, Hget2. split.
-          
-          eexists. split. reflexivity.
-          intros x.
-          destruct (M.get x rho1) as [v1|] eqn:Hgetv1.
-          edestruct Hl as [v2 [Hgetv2 Hi]]; try eassumption.
-          now constructor.
-          left; repeat eexists; eauto. intros. now eapply Hi.
-          destruct (M.get x rho2) as [v2|] eqn:Hgetv2; eauto.
-          edestruct Hr as [v1 [Hgetv1' Hi']]; try eassumption.
-          now constructor. congruence.
-          
-          eexists. split. reflexivity.
-          intros x.
-          destruct (M.get x rho1) as [v1|] eqn:Hgetv1.
-          edestruct Hl as [v2 [Hgetv2 Hi]]; try eassumption.
-          now constructor.
-          left; repeat eexists; eauto. intros. now eapply Hi.
-          destruct (M.get x rho2) as [v2|] eqn:Hgetv2; eauto.
-          edestruct Hr as [v1 [Hgetv1' Hi']]; try eassumption.
-          now constructor. congruence.
-      + destruct (get l2 H2) eqn:Hget2; try contradiction.
-        intros. rewrite !res_approx_fuel_eq. simpl.
-        rewrite Hget1, Hget2; eauto.
-    - split; try contradiction.
-      intros Heq. destruct (Heq 0%nat) as [Hl Hr].
-      rewrite res_approx_fuel_eq in *. contradiction.
-    - split; try contradiction.
-      intros Heq. destruct (Heq 0%nat) as [Hl Hr].
-      rewrite res_approx_fuel_eq in *. contradiction.
-    - split.
-      + intros Heq. destruct (Heq 0%nat) as [Hl Hr].
-        rewrite res_approx_fuel_eq in *. inv Hl. split; eauto.
-      + intros [Hl1 Hr2]; subst.
-        split; eauto; rewrite res_approx_fuel_eq; simpl; split; eauto.  
-  Qed.  
-  
   Definition val_loc (v : value) : Ensemble loc :=
     match v with
       | Loc l => [set l]
@@ -351,7 +55,7 @@ Module HeapDefs (H : Heap).
                         | Some v => val_loc v
                         | None => Empty_set _
                       end).
-
+  
   (** Size of the domain of a map TODO move *)
   Definition size_map {A} (m : M.t A) :=
     List.length (M.elements m).
@@ -361,21 +65,14 @@ Module HeapDefs (H : Heap).
     match v with
       | Constr t ls => (* The size of the constructor representation *)
         1 + length ls
-      | Env rho => (* The size of the record that will represent the environment *)
+      | Env rho =>
         1 + size_map rho
     end.
   
   (** Size of the heap *)
   Definition size_heap (H : heap block) : nat :=
     size_with_measure size_val H.
-
-  (* TODO move *)
-  Fixpoint Union_list {A} (l : list (Ensemble A)) : Ensemble A :=
-    match l with
-      | nil => Empty_set _
-      | cons x xs => x :|: Union_list xs
-    end.
-  
+    
   (** The locations that appear on a block *)
   Definition locs (v : block) : Ensemble loc :=
     match v with
@@ -419,24 +116,6 @@ Module HeapDefs (H : Heap).
   Definition closed (S : Ensemble loc) (H : heap block) : Prop :=
     forall l, l \in S -> exists v, get l H = Some v /\ locs v \subset S.
 
-  
-  (** Using S as the set of roots, garbage collect H1 *) 
-  Definition collect (S : Ensemble loc) (H1 H2 : heap block) : Prop :=
-    size_heap H2 <= size_heap H1 /\
-    S |- H1 ≃ H2. (* locations outside S might be renamed! *)
-  
-  (** [live S H1 H2] iff H2 is the live portion of H1, using S as roots *)
-  Definition live (S : Ensemble loc) (H1 H2 : heap block) : Prop :=
-    size_heap H2 <= size_heap H1 /\ (* maybe could be derived *)
-    heap_equiv S H1 H2 /\ (* locations outside S might be renamed! *)
-    dom H2 \subset reach' H2 S. (* everything in the domain is reachable *)
-
-  (** The size of the reachable portion of the heap *)
-  Definition size_reach (H : heap block) (S : Ensemble loc) (n : nat) : Prop :=
-    forall H', live S H H' -> size_heap H' = n. 
-
-  Import ListNotations.
-
   (** Add a block of function definitions in the heap and the environment *)
   Fixpoint def_closures (B B0: fundefs) (rho : env) (H : heap block) (ct : cTag) (cenv : loc) {struct B}
   : heap block * env :=
@@ -451,38 +130,29 @@ Module HeapDefs (H : Heap).
         (H'', M.set f (Loc l) rho') 
       | Fnil => (H, rho)
     end.
-  
-  (** * Lemmas about [collect] *)
-  
-  (** The reachable part of the heap before and after collection are the same *)
-  Lemma collect_heap_eq S H1 H2 :
-    collect S H1 H2 ->
-    S |- H1 ≃ H2.
-  Proof.
-    firstorder.
-  Qed.
-  
-  Lemma collect_size S H1 H2 :
-    collect S H1 H2 ->
-    size_heap H2 <= size_heap H1.
-  Proof.
-    now firstorder.
-  Qed.
 
+  (* TODO move *)
+  (* M utils *)
+  Definition key_set {A : Type} (map : M.t A) :=
+    [ set x : positive | match M.get x map with
+                           | Some x => True
+                           | None => False
+                         end ].
 
+  Definition sub_map {A : Type} (map1 map2 : M.t A) :=
+    forall x v, M.get x map1 = Some v ->
+           M.get x map2 = Some v.
+  
+  (** [rho'] is the restriction of [rho] in [S] *)
+  Definition restrict_env (S : Ensemble var) (rho rho' : env) : Prop :=
+    (forall x, x \in S -> M.get x rho = M.get x rho') /\
+    sub_map rho' rho /\ key_set rho' \subset S.
+  
   (** * Lemmas about [post] and [reach'] *)
   
 
   (** Set monotonicity lemmas *)
-  
-  Lemma post_heap_monotonic H1 H2 S :
-    H1 ⊑ H2 ->
-    post H1 S \subset post H2 S.
-  Proof.
-    unfold post. intros Hsub l [l' [v [Hin [Hget Hin']]]].
-    exists l', v. split; eauto.
-  Qed.
-  
+    
   Lemma post_set_monotonic S1 S2 H :
     S1 \subset S2 ->
     post H S1 \subset post H S2.
@@ -503,6 +173,14 @@ Module HeapDefs (H : Heap).
   Qed.
 
   (** Heap monotonicity lemmas *)
+
+  Lemma post_heap_monotonic H1 H2 S :
+    H1 ⊑ H2 ->
+    post H1 S \subset post H2 S.
+  Proof.
+    unfold post. intros Hsub l [l' [v [Hin [Hget Hin']]]].
+    exists l', v. split; eauto.
+  Qed.
 
   Lemma post_n_heap_monotonic n (H1 H2 : heap block) (S : Ensemble loc) :
     H1 ⊑ H2 -> (post H1 ^ n) S \subset (post H2 ^ n) S.
@@ -535,6 +213,13 @@ Module HeapDefs (H : Heap).
     intros x Hin. exists 1; split; eauto.
     now constructor.
   Qed.
+
+  Lemma Included_post_n_reach' (H : heap block) (S : Ensemble loc) (n : nat) :
+    (post H ^ n) S \subset reach' H S.
+  Proof.
+    intros l Hp. eexists; eauto. split; eauto. constructor.
+  Qed.
+  
   
   Lemma reach_unfold H S :
     (reach' H S) <--> (Union _ S (reach' H (post H S))).
@@ -589,13 +274,6 @@ Module HeapDefs (H : Heap).
       exists 0. split; eauto. now constructor.
   Qed.
 
-  (* Lemma reach'_env_set S H v rho x : *)
-  (*   val_loc v \in reach' H (env_locs rho (S \\ [set x])) -> *)
-  (*   reach' H (env_locs rho (S \\ [set x])) <--> *)
-  (*   reach' H (env_locs (M.set x v rho) S). *)
-  (* Proof with now eauto with Ensembles_DB. *)
-  (*   intros Hin. *)
-  (* Abort. *)
 
   (* TODO better name for this? *)
   Lemma reach_spec H S S' :
@@ -686,7 +364,7 @@ Module HeapDefs (H : Heap).
     now apply Included_post_reach'.
   Qed.
   
-  (** Union lemmas *)
+  (** Set lemmas *)
 
   Lemma post_Union H S1 S2 :
     post H (Union _ S1 S2) <--> Union _ (post H S1) (post H S2).
@@ -726,6 +404,7 @@ Module HeapDefs (H : Heap).
       repeat eexists; eauto; eapply post_n_Union; eauto.
   Qed.
 
+
   (** Disjointedness lemmas *)
 
   Lemma post_Disjoint S H :
@@ -758,7 +437,7 @@ Module HeapDefs (H : Heap).
      - intros l [n [_ Hp]]. eapply post_n_Disjoint; eauto.
      - apply reach'_extensive.
    Qed.
-
+   
   (** allocation lemmas *)
    
   Lemma post_alloc S H v l H'  :
@@ -809,15 +488,18 @@ Module HeapDefs (H : Heap).
     - eapply reach'_heap_monotonic. now eapply alloc_subheap; eauto.
   Qed.
 
+  (** Decidability lemmas *)
+
   (** TODO implement BFS in the heap to find reachable locs *)
   Lemma Decidable_reach' (S : Ensemble loc) (H : heap block) :
     Decidable S ->
     Decidable (reach' H S).
   Admitted.
+  
 
   (** * Lemmas about [env_locs] *)
   
-  (* XXX move *)
+  (* TODO move *)
   Lemma image'_monotonic {A B} (S1 S2 : Ensemble A) (f : A -> option B) :
     S1 \subset S2 ->
     image' f S1 \subset image' f S2.
@@ -902,19 +584,54 @@ Module HeapDefs (H : Heap).
         constructor; eauto. intros Heq. inv Heq; congruence. 
   Qed.
 
-  (* XXX fix *)
-  (* Lemma env_locs_def_funs_Included B l rho S : *)
-  (*   env_locs (def_funs B l rho) *)
-  (*            (Union M.elt S (name_in_fundefs B)) \subset *)
-  (*            Union _ (env_locs rho S) [set l]. *)
-  (* Proof. *)
-  (*   induction B; simpl. *)
-  (*   - eapply Included_trans. *)
-  (*     rewrite (Union_commut [set v]), Union_assoc. *)
-  (*     eapply env_locs_set_Inlcuded. rewrite Union_commut. *)
-  (*     eapply Union_Included; eauto with Ensembles_DB. *)
-  (*   - rewrite Union_Empty_set_neut_r; eauto with Ensembles_DB. *)
-  (* Qed. *)
+  (* name? *)
+  Lemma env_locs_singleton_Included (x : var) (v : value) (rho : env)
+          (S : Ensemble var):
+    (val_loc v) \subset env_locs (M.set x v rho) (Union _ S [set x]).
+  Proof.
+    rewrite env_locs_set_In; eauto with Ensembles_DB.
+  Qed.
+
+  
+  Lemma def_closures_env_locs_in_dom S H H' rho rho' B B0 ct l :
+    def_closures B B0 rho H ct l = (H', rho') ->
+    env_locs rho S \subset dom H ->
+    env_locs rho' (S :|: name_in_fundefs B) \subset dom H'.
+  Proof.
+    revert S rho rho' H H'; induction B; intros S rho rho' H H' Hdef Hsub; simpl.
+    - simpl in Hdef.
+      destruct (def_closures B B0 rho H ct l) as [H'' rho''] eqn:Hdef'.
+      destruct (alloc _ H'') as [l' H'''] eqn:Hal. inv Hdef.
+      rewrite alloc_dom; [| eassumption ].
+      rewrite env_locs_set_In; [| now eauto with Ensembles_DB ].
+      simpl. eapply Included_Union_compat.
+      reflexivity.
+      eapply Included_trans; [| eapply IHB; eassumption ].
+      eapply env_locs_monotonic.
+      now eauto with Ensembles_DB.
+    - rewrite Union_Empty_set_neut_r. inv Hdef. eassumption.
+  Qed.
+
+  Lemma env_locs_def_funs S S1 H1 H1' rho1 rho1'  B B0 c l :
+    env_locs rho1 (Setminus _ S (name_in_fundefs B)) \subset S1 ->
+    l \in S1 ->
+    (H1', rho1') = def_closures B B0 rho1 H1 c l ->
+    env_locs rho1' (Setminus _ S (name_in_fundefs B)) \subset S1.
+  Proof.
+    revert S H1' rho1'; induction B; intros S H1' rho1' Hsub1 Hsub2 Heq.
+    - simpl in Heq. destruct (def_closures B B0 rho1 H1 c l) as [H'' rho''].
+      destruct (alloc _ H'') as [l' H'''] eqn:Heq'.
+      inv Heq. rewrite env_locs_set_not_In.
+      simpl; rewrite <- !Setminus_Union.
+      simpl in Hsub1; rewrite <- !Setminus_Union in Hsub1.
+      eapply IHB; eauto.
+      intros Hc. inversion Hc as [Hc1 Hc2]; eauto. 
+      eapply Hc2; left; eauto.
+    - simpl in Hsub1.
+      rewrite Setminus_Empty_set_neut_r in Hsub1; inv Heq.
+      rewrite Setminus_Empty_set_neut_r; eauto.
+  Qed.
+
   
   Lemma env_locs_setlist_Included ys ls rho rho' S :
     setlist ys ls rho = Some rho'  ->
@@ -933,6 +650,8 @@ Module HeapDefs (H : Heap).
       eapply Included_trans. eapply IHys; eauto.
       now eauto with Ensembles_DB. 
   Qed.
+
+  (* Decidability lemmas *)
 
   Lemma Decidable_val_loc v :
     Decidable (val_loc v).
@@ -982,7 +701,8 @@ Module HeapDefs (H : Heap).
       eapply M.elements_correct; eassumption.
   Qed.
   
-  (* Set lemmas *)
+  (** Set lemmas *)
+
   Lemma env_locs_Union rho S1 S2 :
     env_locs rho (Union _ S1 S2) <-->
     Union _ (env_locs rho S1) (env_locs rho S2).
@@ -996,14 +716,13 @@ Module HeapDefs (H : Heap).
       right; eauto.
   Qed.
 
-  Lemma env_locs_Empty S :
-    Empty_set _ <--> env_locs (M.empty _) S.
+  Lemma env_locs_Empty_set (rho : env) :
+    env_locs rho (Empty_set _) <--> Empty_set _.
   Proof.
-    split; eauto with Ensembles_DB.
-    intros l [v [Hs Hp]]. rewrite M.gempty in Hp.
-    inv Hp.
+    unfold env_locs. rewrite big_cup_Empty_set.
+    reflexivity.
   Qed.
-
+  
   Lemma env_locs_Singleton x rho v :
     M.get x rho = Some v ->
     env_locs rho [set x] <--> (val_loc v).
@@ -1023,19 +742,15 @@ Module HeapDefs (H : Heap).
     rewrite M.gss; eauto.
   Qed.
   
-  Lemma env_locs_singleton_Included (x : var) (v : value) (rho : env)
-        (S : Ensemble var):
-    (val_loc v) \subset env_locs (M.set x v rho) (Union _ S [set x]).
+  Lemma env_locs_Empty S :
+    Empty_set _ <--> env_locs (M.empty _) S.
   Proof.
-    rewrite env_locs_set_In; eauto with Ensembles_DB.
+    split; eauto with Ensembles_DB.
+    intros l [v [Hs Hp]]. rewrite M.gempty in Hp.
+    inv Hp.
   Qed.
 
-  Lemma env_locs_Empty_set (rho : env) :
-    env_locs rho (Empty_set _) <--> Empty_set _.
-  Proof.
-    unfold env_locs. rewrite big_cup_Empty_set.
-    reflexivity.
-  Qed.
+  (* get lemmas *)
 
   Lemma env_locs_FromList (rho : env) (xs : list var) (vs : list value) :
     getlist xs rho = Some vs ->
@@ -1052,7 +767,7 @@ Module HeapDefs (H : Heap).
       eapply env_locs_Singleton. eassumption.
       eapply IHxs. reflexivity.
   Qed.
-
+  
   (* XXX fix *)
   (* Lemma reach_env_locs_alloc (S : Ensemble var) (H H' : heap block) (rho : env) *)
   (*       (x : var) (v : value) (b : block) : *)
@@ -1074,6 +789,8 @@ Module HeapDefs (H : Heap).
   (*     eapply reach'_extensive. *)
   (*   - right. rewrite <- reach'_alloc; eauto. *)
   (* Qed. *)
+
+  (** get lemmas *)
 
   Lemma get_In_env_locs x S rho v:
     x \in S ->
@@ -1101,9 +818,97 @@ Module HeapDefs (H : Heap).
       + eapply IHxs; eauto.
         eapply Included_trans...
   Qed.
+
+  Lemma reach_env_locs_alloc_not_In S H H' rho x b l :
+    alloc b H = (l, H') ->
+    locs b \subset (reach' H (env_locs rho S)) ->
+    ~ x \in S ->
+    Union _ [set l] (reach' H (env_locs rho S)) \subset
+    reach' H' (env_locs (M.set x (Loc l) rho) (Union _ S [set x])).
+  Proof.
+    intros Hal Hsub Hnin l1 Hin.
+    rewrite <- (env_locs_set_not_In) with (l := Loc l) in Hin; eauto.
+    rewrite env_locs_Union, reach'_Union. inv Hin.
+    - inv H0. right. exists 0. split. 
+      now constructor. simpl. eexists. split; eauto.
+      reflexivity. now rewrite M.gss.
+    - left. eapply reach'_heap_monotonic; eauto.
+      eapply alloc_subheap. eassumption.
+  Qed.
+
+  Lemma restrict_env_env_locs rho rho' S :
+    restrict_env S rho rho' ->
+    env_locs rho' (Full_set _) \subset env_locs rho S. 
+  Proof.
+    intros [H1 [H2 H3]] l [x [_ H]].
+    destruct (M.get x rho') eqn:Hget; try contradiction.
+    exists x. split.
+    eapply H3. unfold key_set, In. now rewrite Hget.
+    eapply H2 in Hget. now rewrite Hget.
+  Qed.    
+
+
+  (** * Lemmas about [def_closures] *)
+
+  Lemma def_funs_subheap H H' rho rho' B B0 c l :
+    (H', rho') = def_closures B B0 rho H c l ->
+    H ⊑ H'.
+  Proof.
+    revert H' rho'; induction B; intros H' rho' Heq;
+    simpl; [| inv Heq; now apply subheap_refl ].
+    simpl in Heq. destruct (def_closures B B0 rho H c l) as [H'' rho''].
+    destruct (alloc _ H'') as [l' H'''] eqn:Heq'.
+    inv Heq. eapply subheap_trans; eauto.
+    now eapply alloc_subheap; eauto.
+  Qed.
+
+
+  Lemma def_closures_post_reach
+        (S : Ensemble var) (H H' : heap block) (rho rho' : env)
+        (B B0 : fundefs) (ct : cTag) (l : loc) :
+    def_closures B B0 rho H ct l = (H', rho') ->
+    post H [set l] \subset (reach' H (env_locs rho S)) ->
+    post H' [set l] \subset (reach' H' (env_locs rho' (S :|: name_in_fundefs B))).
+  Proof.
+    revert S rho rho' H H'; induction B; intros S rho rho' H H' Hdef Hsub; simpl.
+    - simpl in Hdef.
+      destruct (def_closures B B0 rho H ct l) as [H'' rho''] eqn:Hdef'.
+      destruct (alloc _ H'') as [l' H'''] eqn:Hal. inv Hdef.
+      intros l1 [l2 [b2 [Hin1 [Hget2 Hin2]]]]. inv Hin1. 
+      exists 2. split. constructor.
+      exists l2. eexists. split. simpl.
+      eexists l'. eexists. split. simpl.
+      eexists v. split. right. left. reflexivity.
+      rewrite M.gss. reflexivity.
+      split. eapply gas; eassumption.
+      simpl. right. left. reflexivity.
+      split; eauto.
+    - rewrite Union_Empty_set_neut_r. inv Hdef.
+      eassumption.
+  Qed.
+
+  Lemma def_closures_env_reach S H H' rho rho' B B0 ct l :
+    def_closures B B0 rho H ct l = (H', rho') ->
+    l \in (reach' H (env_locs rho S)) ->
+    l \in (reach' H' (env_locs rho' (S :|: name_in_fundefs B))).
+  Proof.
+    revert S rho rho' H H'; induction B; intros S rho rho' H H' Hdef Hin; simpl.
+    - simpl in Hdef.
+      destruct (def_closures B B0 rho H ct l) as [H'' rho''] eqn:Hdef'.
+      destruct (alloc _ H'') as [l' H'''] eqn:Hal. inv Hdef.
+      exists 1. split. constructor.
+      exists l'. eexists. split. simpl.
+      eexists v. split. right. left. reflexivity.
+      rewrite M.gss. reflexivity.
+      split. eapply gas; eassumption.
+      simpl. right. left. reflexivity.
+    - rewrite Union_Empty_set_neut_r. inv Hdef.
+      eassumption.
+  Qed.
+
   
   (** * Lemmas about locs *)
-
+  
   (* TODO move *)
   Instance Decidable_FromList A (H : forall (x y : A), {x = y} + {x <> y}) (l : list A) :
     Decidable (FromList l).
@@ -1116,6 +921,7 @@ Module HeapDefs (H : Heap).
         right. intros Hc. inv Hc; eauto.
   Qed.
 
+  (* TODO move *)
   Instance Decidable_map_UnionList {A B : Type} (f : A -> Ensemble B) (H : forall x, Decidable (f x)) l :
     Decidable (Union_list (map f l)).
   Proof.
@@ -1140,25 +946,11 @@ Module HeapDefs (H : Heap).
   Qed.  
   
 
-  (** * Lemmas about [reach_size] *)
-
-(*
-  Lemma size_reach_heap_eq (S : Ensemble loc) (H1 H1' : heap block) (m : nat) :
-    reach' H1 S |- H1 ≡ H1' ->
-    size_reach H1 S m ->
-    size_reach H1' S m.
-  Proof.
-    intros Heq Hs H2 Hl. eapply Hs.
-    eapply live_heap_eq; eauto. rewrite <- reach'_heap_eq; eauto.
-    now symmetry.
-  Qed.
- *)
-
   (** * Lemmas about [closed] *)
 
   Lemma in_dom_closed (S : Ensemble loc) (H : heap block) :
-    closed (reach' H S) H ->
-    (reach' H S) \subset dom H.
+    closed S H ->
+    S \subset dom H.
   Proof. 
     intros Hc l1 Hr.
     edestruct Hc as [v2 [Hget' Hdom]]; eauto.
@@ -1175,7 +967,7 @@ Module HeapDefs (H : Heap).
       [| now eapply reach'_post_fixed_point_n with (n := 1)]; simpl.
     intros l' Hin'. do 2 eexists. split. eassumption. now split; eauto.
   Qed.
-
+  
   Lemma closed_alloc H H' l v :
     closed (dom H) H ->
     locs v \subset dom H ->
@@ -1203,7 +995,7 @@ Module HeapDefs (H : Heap).
     - setoid_rewrite <- Heq; eauto.
     - setoid_rewrite Heq; eauto.
   Qed.
-
+  
   Lemma closed_Union (S1 S2 : Ensemble loc) (H : heap block) :
     closed S1 H ->
     closed S2 H ->
@@ -1217,6 +1009,106 @@ Module HeapDefs (H : Heap).
       eexists; split; eauto...
   Qed.
 
+  Lemma closed_alloc' S H H' l v :
+    closed S H ->
+    locs v \subset S ->
+    alloc v H = (l, H') ->
+    closed S H'.
+  Proof with now eauto with Ensembles_DB.
+    intros Hcl Hin Ha l1 Hin'.
+    destruct (loc_dec l1 l); subst.
+    - eexists. erewrite gas; eauto.
+    - edestruct Hcl as [l2 [Hget Hsub]]; try eassumption.
+      eexists. erewrite gao; eauto; split; eauto.
+  Qed.
+
+  Lemma closed_alloc_Union S H H' l v :
+    closed S H ->
+    locs v \subset S ->
+    alloc v H = (l, H') ->
+    closed (l |: S) H'.
+  Proof with now eauto with Ensembles_DB.
+    intros Hcl Hin Ha l1 Hin'.
+    destruct (loc_dec l1 l); subst.
+    - eexists. erewrite gas; eauto. split; eauto...
+    - inv Hin'. inv H0. contradiction.
+      edestruct Hcl as [l2 [Hget Hsub]]; try eassumption.
+      eexists. erewrite gao; eauto; split; eauto...
+  Qed.
+
+  Lemma closed_def_funs S1 H1 H1' rho1 rho1'  B B0 c l :
+    closed S1 H1 ->
+    l \in S1 ->
+    (H1', rho1') = def_closures B B0 rho1 H1 c l ->
+    closed S1 H1'.
+  Proof.
+    revert H1' rho1'; induction B;
+    intros H1' rho1' Hc Hsub Heq; [| inv Heq; now eauto ].
+    simpl in Heq. destruct (def_closures B B0 rho1 H1 c l) as [H'' rho''].
+    destruct (alloc _ H'') as [l' H'''] eqn:Heq'.
+    inv Heq. eapply closed_alloc'; [| | eassumption ]; eauto.
+    simpl. rewrite Union_Empty_set_neut_r, Union_Empty_set_neut_l.
+    eapply Singleton_Included. eassumption.
+  Qed.
+  
+  Lemma def_funs_exists_new_set S S1 H1 H1' rho1 rho1' rho_clo B B0 c l :
+    closed S1 H1 ->
+    env_locs rho1 (Setminus _ S (name_in_fundefs B)) \subset S1 ->
+    get l H1 = Some (Env rho_clo) ->
+    env_locs rho_clo (Full_set _) \subset S1 ->
+    (H1', rho1') = def_closures B B0 rho1 H1 c l ->
+    exists S1', S1 \subset S1' /\ closed S1' H1' /\
+           env_locs rho1' S \subset S1'.
+  Proof with now eauto with Ensembles_DB.
+    revert S H1' rho1'; induction B; intros S H1' rho1' Hc Henv Hget Hsub Heq.
+    - simpl in Heq. destruct (def_closures B B0 rho1 H1 c l) as [H'' rho''] eqn:Hdef.
+      destruct (alloc _ H'') as [l' H'''] eqn:Heq'.
+      inv Heq.
+      edestruct IHB as [S1' [Hsub' [Hc' Henv']]]; eauto.
+      eapply Included_trans; [| now apply Henv ].
+      eapply env_locs_monotonic. simpl. rewrite <- !Setminus_Union.
+      reflexivity.
+      eexists (l' |: (l |: S1')). split. 
+      now eauto with Ensembles_DB.
+      split.
+      + eapply closed_alloc_Union; [| | eassumption ];
+        simpl; try now eauto with Ensembles_DB.
+        intros l1 Hin; inv Hin.
+        * inv H. eexists.
+          split. eapply def_funs_subheap; now eauto.
+          eapply Included_trans. eassumption. now eauto with Ensembles_DB.
+        * eapply Hc' in H. destruct H as [v' [Hgetv HsubS]].
+          eexists. split; eauto.
+          eapply Included_trans...
+      + eapply Included_trans. now eapply env_locs_set_Inlcuded'.
+        now eauto with Ensembles_DB.
+    - simpl in Henv.
+      rewrite Setminus_Empty_set_neut_r in Henv; inv Heq.
+      eexists. split; eauto. reflexivity.
+  Qed.
+
+  Lemma closed_post_n_in_S (S : Ensemble loc) (H : heap block) (n : nat) :
+    closed S H ->
+    (post H ^ n) S \subset S.
+  Proof. 
+    induction n; intros Hc l1 Hr.
+    - eassumption.
+    - edestruct Hr as [l2 [b [Hin1 [Hget Hin2]]]]; eauto.
+      eapply IHn in Hin1; [| eassumption ].
+      edestruct Hc as [b1 [Hget2 Hsub]]; try eassumption.
+      subst_exp. eapply Hsub. eassumption.
+  Qed.
+
+  Lemma closed_reach_in_S (S : Ensemble loc) (H : heap block) :
+    closed S H ->
+    reach' H S \subset S.
+  Proof. 
+    intros Hc l1 Hr.
+    edestruct Hr as [n [_ Hr']].
+    eapply closed_post_n_in_S; eauto.
+  Qed.
+
+  
   (** * Lemmas about [well_formed] and [well_formed_env] *)
   
   (** Monotonicity lemmas *)
@@ -1308,7 +1200,7 @@ Module HeapDefs (H : Heap).
     eapply reachable_closed; eauto.
   Qed.
 
-  (* XXX mvove *)
+  (* TODO move *)
     
   Lemma getlist_in_dom (S : Ensemble var) (H : heap block) (rho : env)
         (ys : list var) (vs : list value) :
@@ -1332,63 +1224,6 @@ Module HeapDefs (H : Heap).
   (** Well-formedness preservation under environment and heap extensions *)
 
   (** Allocation lemmas *)
-
-  Lemma closed_set_alloc_alt S H H' b l rho x :
-    closed (reach' H (env_locs rho (S \\ [set x]))) H ->
-    locs b \subset (reach' H (env_locs rho (S \\ [set x]))) ->
-    alloc b H = (l, H') ->
-    closed (reach' H' (env_locs (M.set x (Loc l) rho) S)) H'.
-  Proof with now eauto with Ensembles_DB.
-    intros Hcl Hin Ha l1 Hin'.
-    destruct (loc_dec l1 l); subst.
-    - eexists. erewrite gas; eauto.
-      split. reflexivity.
-      eapply Included_trans. eassumption.
-      eapply Included_trans.
-      eapply reach'_heap_monotonic.
-      now eapply alloc_subheap; eauto.
-      eapply reach'_set_monotonic.
-      rewrite <- env_locs_set_not_In.
-      eapply env_locs_monotonic...
-      intros Hinx. now inv Hinx; eauto.
-    - eapply reach'_set_monotonic in Hin';
-      [| now eapply env_locs_set_Inlcuded'].
-      rewrite reach'_Union in Hin'.
-      rewrite reach_unfold in Hin'.
-      simpl in Hin'. rewrite post_Singleton in Hin'; [| now erewrite gas; eauto ].
-      inv Hin'.
-      + inv H0.
-        * inv H1. congruence.
-        * edestruct Hcl as [b1 [Hget1 Hsub]]; eauto.
-          rewrite <- reach'_alloc; try eassumption.
-          rewrite reach'_idempotent.
-          eapply reach'_set_monotonic; [| eassumption ].
-          eapply Included_trans. eassumption.
-          eapply reach'_heap_monotonic.
-          eapply alloc_subheap. eassumption.
-          eexists; split; eauto.
-          
-          now erewrite gao; eauto.
-          
-          eapply Included_trans. eassumption.
-          eapply Included_trans. eapply reach'_heap_monotonic.
-          eapply alloc_subheap. eassumption.
-          eapply reach'_set_monotonic. 
-          rewrite <- env_locs_set_not_In.
-          eapply env_locs_monotonic...
-          intros Hc. inv Hc; eauto.            
-      + edestruct Hcl as [b1 [Hget1 Hsub]]; eauto.
-        rewrite <- reach'_alloc; try eassumption.
-        eexists.
-        erewrite gao; eauto; split; eauto.
-        eapply Included_trans. eassumption.
-        eapply Included_trans. eapply reach'_heap_monotonic.
-        eapply alloc_subheap. eassumption.
-        eapply reach'_set_monotonic. 
-        rewrite <- env_locs_set_not_In.
-        eapply env_locs_monotonic...
-        intros Hc. inv Hc; eauto.
-  Qed.
   
   Lemma well_formed_alloc (S : Ensemble loc) (H H' : heap block)
              (b : block) (l : loc) :
@@ -1476,28 +1311,22 @@ Module HeapDefs (H : Heap).
     rewrite reach'_Union. eapply well_formed_Union; eauto.
   Qed.
   
-  (* XXX fix *)
-  (* Lemma well_formed_reach_alloc_def_funs S H B l v H' rho : *)
-  (*   well_formed (reach' H (env_locs rho S)) H -> *)
-  (*   env_locs rho S \subset dom H -> *)
-  (*   alloc v H = (l, H') -> *)
-  (*   locs v \subset (reach' H (env_locs rho S)) -> *)
-  (*   well_formed (reach' H' (env_locs (def_funs B l rho) (Union _ S (name_in_fundefs B)))) H'. *)
-  (* Proof with now eauto with Ensembles_DB. *)
-  (*   induction B; intros Hwf Hsub Ha Hin; simpl. *)
-  (*   - rewrite (Union_commut [set v0]), Union_assoc. *)
-  (*     eapply well_formed_reach_set. *)
-  (*     + eapply IHB; eauto. *)
-  (*     + eapply well_formed_antimon. *)
-  (*       eapply reach'_set_monotonic. *)
-  (*       now apply env_locs_singleton_Included with (x := v0). *)
-  (*       eapply well_formed_reach_alloc; eauto. *)
-  (*   - rewrite Union_Empty_set_neut_r. *)
-  (*     rewrite reach'_alloc; eauto. *)
-  (*     eapply well_formed_alloc; eauto. *)
-  (*     eapply Included_trans. eassumption. *)
-  (*     eapply reachable_in_dom; eauto. *)
-  (* Qed. *)
+  Lemma well_formed_def_funs S1 H1 H1' rho1 rho1'  B B0 c l :
+    well_formed S1 H1 ->
+    l \in dom H1 ->
+    (H1', rho1') = def_closures B B0 rho1 H1 c l ->
+    well_formed S1 H1'.
+  Proof.
+    revert H1' rho1'; induction B;
+    intros H1' rho1' Hc Hsub Heq; [| inv Heq; now eauto ].
+    simpl in Heq. destruct (def_closures B B0 rho1 H1 c l) as [H'' rho''] eqn:Hdef.
+    destruct (alloc _ H'') as [l' H'''] eqn:Heq'.
+    inv Heq. eapply well_formed_alloc; [| eassumption | ]; eauto.
+    simpl. rewrite Union_Empty_set_neut_r, Union_Empty_set_neut_l.
+    eapply Singleton_Included.
+    eapply dom_subheap. eapply def_funs_subheap; eauto.
+    eassumption.
+  Qed.
 
   Lemma well_formed_reach_setlist  (S : Ensemble M.elt) (H : heap block) 
         (rho rho' : env)  (xs : list M.elt) (vs : list value) :
@@ -1537,7 +1366,174 @@ Module HeapDefs (H : Heap).
     rewrite <- reach'_idempotent. eassumption.
   Qed.   
 
-  (* TODO move? *)
+     
+  Lemma well_formed_post_n_alloc_same (S : Ensemble loc) (H H' : heap block)
+        b l n :
+    well_formed (reach' H S) H  ->
+    S \subset dom H ->
+    alloc b H = (l, H') ->
+    (post H ^ n) S <--> (post H' ^ n) S.
+  Proof.
+    intros Hwf Hdom Hal. split; intros l' Hin.
+    - revert l' Hin; induction n; simpl in *; intros l' Hin.
+      + eassumption.
+      + destruct Hin as [l'' [b' [Hin [Hget Hin']]]].
+        eapply IHn in Hin.
+        eexists. eexists. split. eassumption.
+        split; [| eassumption ].
+        erewrite gao; try eassumption.
+        intros Heq; subst. 
+        erewrite alloc_fresh in Hget; try eassumption.
+        discriminate.
+    - revert l' Hin; induction n; simpl in *; intros l' Hin.
+      + eassumption.
+      + destruct Hin as [l'' [b' [Hin [Hget Hin']]]].
+        eapply IHn in Hin.
+        eexists. eexists. split. eassumption.
+        split; [| eassumption ].
+        eapply reachable_in_dom in Hdom; [| eassumption ].
+        edestruct Hdom as [b'' Hget''].
+        eexists; split; [| exact Hin ]. now constructor.
+        erewrite gao in Hget; try eassumption.
+        intros Heq; subst.
+        erewrite alloc_fresh in Hget''; try eassumption.
+        discriminate.
+  Qed.
+
+  Lemma well_formed_reach_alloc_same (S : Ensemble loc) (H H' : heap block)
+        b l :
+    well_formed (reach' H S) H  ->
+    S \subset dom H ->
+    alloc b H = (l, H') ->
+    reach' H S <--> reach' H' S.
+  Proof.
+    intros Hwf Hdom Hal. split; intros l' [n [_ Hin]].
+    - eapply (well_formed_post_n_alloc_same S H H') in Hin; eauto.
+      eexists; split; eauto. constructor.
+    - eapply (well_formed_post_n_alloc_same S H H') in Hin; eauto.
+      eexists; split; eauto. constructor.
+  Qed.
+
+  Lemma well_formed_reach_def_closed_same (S : Ensemble loc) (H H' : heap block) B B0 rho rho' ct l :
+    well_formed (reach' H S) H  ->
+    In loc (dom H) l ->
+    S \subset dom H ->
+    def_closures B B0 rho H ct l = (H', rho') ->
+    reach' H S <--> reach' H' S.
+  Proof.
+    intros Hwf Hdom HS; revert H' rho'; induction B; intros H' rho' Hdef. 
+    - simpl in Hdef.
+      destruct (def_closures B B0 rho H ct ) as [H'' rho''] eqn:Hdef'.
+      destruct (alloc _ H'') as [l' H'''] eqn:Ha. inv Hdef.
+      assert (Heq :reach' H'' S <--> reach' H' S).
+      { eapply well_formed_reach_alloc_same; eauto.
+        eapply well_formed_def_funs; eauto.
+        rewrite <- IHB; [| reflexivity ]. eassumption.
+        eapply Included_trans. eassumption.
+        eapply dom_subheap. eapply def_funs_subheap.
+        eauto. }
+      rewrite <- Heq, IHB; reflexivity.
+    - inv Hdef. reflexivity.
+  Qed.
+  
+  Lemma well_formed_reach_alloc_in_dom (S : Ensemble var) (H H' : heap block)
+        (rho : env) (x : var) (b : block) (l : loc) :
+    well_formed (reach' H (env_locs rho S)) H  ->
+    env_locs rho S \subset dom H ->
+    post H (locs b) \subset reach' H (env_locs rho S) ->
+    alloc b H = (l, H') ->
+    locs b \subset dom H ->
+    well_formed (reach' H' (env_locs (M.set x (Loc l) rho) (Union _ S [set x]))) H'.
+  Proof with now eauto with Ensembles_DB.
+    intros Hwf Hsub Hpost Ha Hin.
+    intros l1 b1 Hin1 Hget.
+    destruct (loc_dec l l1); subst.
+    - erewrite gas in Hget; eauto. inv Hget.
+      eapply Included_trans. eassumption.
+      eapply dom_subheap. eapply alloc_subheap. eassumption.
+    - erewrite gao in Hget; eauto.
+      rewrite env_locs_set_In in Hin1; [| now eauto with Ensembles_DB ].
+      rewrite reach'_Union in Hin1.
+      rewrite <- (well_formed_reach_alloc_same (env_locs _ _)) in Hin1; try eassumption.
+      + inv Hin1.
+        * rewrite reach_unfold in H0. inv H0.
+          inv H1. contradiction.
+          simpl in H1. rewrite post_Singleton in H1; [| now erewrite gas; eauto ].
+          rewrite reach_unfold in H1. inv H1.
+          { eapply Included_trans; [| now eapply dom_subheap; eapply alloc_subheap; eauto ].
+            assert (Has : locs b1 \subset post H (locs b)).
+            { intros l' Hlocs. eexists. eexists.
+              split. eassumption. split. eassumption. eassumption. }
+            eapply Included_trans. eassumption.
+            eapply Included_trans. eassumption.
+            eapply reachable_in_dom; eassumption.  }
+          { assert (Heqp : post H (locs b) <--> post H' (locs b)).
+            { eapply well_formed_post_n_alloc_same with (n := 1); try eassumption.
+              rewrite reach_unfold. eapply well_formed_Union.
+              intros l2 b2 Hin2 Hget2.
+              assert (Has : locs b2 \subset post H (locs b)).
+            { intros l' Hlocs. eexists. eexists.
+              split. eassumption. split. eassumption. eassumption. }
+            eapply Included_trans. eassumption.
+            eapply Included_trans. eassumption.
+            eapply reachable_in_dom; eassumption.
+            eapply well_formed_antimon; [| eassumption ].
+            rewrite (reach'_idempotent _ (env_locs rho S)).
+            eapply reach'_set_monotonic. eassumption. }
+            rewrite <- Heqp in H0.
+            eapply well_formed_reach_alloc_same in H0; try eassumption.
+            eapply Included_trans;
+              [| now eapply dom_subheap; eapply alloc_subheap; eauto ].
+            eapply Hwf; try eassumption.
+            eapply reach'_idempotent. eapply reach'_set_monotonic; [| eassumption ].
+            eassumption.
+            eapply well_formed_antimon; [| eassumption ].
+            rewrite (reach'_idempotent _ (env_locs rho S)).
+            eapply reach'_set_monotonic. eassumption.
+            eapply Included_trans; [| eapply reachable_in_dom ]; eauto. }
+        * eapply Included_trans;
+          [| now eapply dom_subheap; eapply alloc_subheap; eauto ].
+          eapply Hwf; try eassumption.
+          eapply reach'_set_monotonic; [| eassumption ]...
+      + eapply well_formed_antimon; [| eassumption ].
+        eapply reach'_set_monotonic.
+        eapply env_locs_monotonic...
+      + eapply Included_trans; [| exact Hsub ].
+        eapply env_locs_monotonic...
+  Qed.
+
+  Lemma well_formed_reach_alloc_def_funs S H H' rho rho' B B0 l ct rho_clo :
+    well_formed (reach' H (env_locs rho S)) H ->
+    env_locs rho S \subset dom H ->
+    get l H = Some (Env rho_clo) ->
+    env_locs rho_clo (Full_set _ ) \subset (reach' H (env_locs rho S)) ->
+    def_closures B B0 rho H ct l = (H', rho') ->
+    well_formed (reach' H' (env_locs rho' (Union _ S (name_in_fundefs B)))) H'.
+  Proof with now eauto with Ensembles_DB.
+    revert rho rho' H H'; induction B; intros rho rho' H H' Hwf Hsub Hget Hlocs Hdef; simpl.
+    - simpl in Hdef.
+      destruct (def_closures B B0 rho H ct l) as [H'' rho''] eqn:Hdef'.
+      destruct (alloc _ H'') as [l' H'''] eqn:Hal. inv Hdef.
+      rewrite (Union_commut [set v]), Union_assoc.
+      eapply well_formed_reach_alloc_in_dom; [| | | eassumption |].
+      + eapply IHB; eassumption.
+      + eapply def_closures_env_locs_in_dom; eauto.
+      + simpl. rewrite Union_Empty_set_neut_l, Union_Empty_set_neut_r.
+        rewrite post_Singleton with (b := Env rho_clo).
+        * simpl. intros l1 Hin.
+          eapply def_closures_post_reach. eassumption.
+          rewrite post_Singleton; eauto. simpl. eassumption.
+          rewrite post_Singleton with (b := Env rho_clo).
+          eassumption. eapply def_funs_subheap; eauto.
+        * eapply def_funs_subheap; eauto.
+      +  eapply Included_trans;
+        [| now eapply dom_subheap; eapply def_funs_subheap; eauto ].
+         simpl. rewrite Union_Empty_set_neut_r, Union_Empty_set_neut_l.
+         eapply Singleton_Included. eexists; eauto.
+    - inv Hdef. rewrite Union_Empty_set_neut_r. eassumption.
+  Qed.
+
+
   Lemma closed_set_alloc S H H' b l rho x :
     closed (reach' H (locs b :|: (env_locs rho (S \\ [set x])))) H ->
     alloc b H = (l, H') ->
@@ -1583,939 +1579,76 @@ Module HeapDefs (H : Heap).
         eapply Included_trans; [| now eapply reach'_extensive ]...
   Qed.    
 
-  (** * Lemmas about [res_approx] and [res_equiv] *)
-
-  (** Preorder and equivalence properties of [res_approx] and [res_equiv] *)
-
-  Lemma heap_equiv_res_approx (S : Ensemble loc) (H1 H2 : heap block)
-        (v : value) (n : nat) :
-    S |- H1 ≃ H2  ->
-    (val_loc v) \subset S -> 
-    res_approx_fuel n (v, H1) (v, H2).
-  Proof.
-    intros [Heq1 Heq2] Hin.
-    destruct v as [l | B f]; rewrite res_approx_fuel_eq; [| now split; eauto ].
-    simpl; destruct (get l H1) eqn:Hget; eauto.
-    eapply Heq1 in Hget; eauto.
-    destruct Hget as [b2 [Hget2 Heq]].
-    destruct b; destruct b2; try contradiction.
-    - destruct Heq as [Heq Hin2]; subst. eexists; split; eauto. 
-      intros. 
-      eapply Forall2_monotonic; eauto. simpl.
-      intros ? ? [Ha1 Ha2]; eauto.
-    - eexists; split; eauto. 
-      intros x. destruct Heq as [Hal Har].
-      destruct (M.get x e) eqn:Hgetx1; destruct (M.get x e0) eqn:Hgetx2;
-      simpl in *; eauto.
-      + left. repeat eexists; eauto.
-        edestruct Hal as [l' [Hgetx2' Ha]]; eauto.
-        now constructor. subst_exp. intros i Hleq; destruct (Ha i); eassumption.
-      + edestruct Hal as [l' [Hgetx2' Ha]]; eauto.
-        now constructor. congruence.
-      + edestruct Har as [l' [Hgetx2' Ha]]; eauto.
-        now constructor. congruence.
-    - eapply Hin. reflexivity. 
-  Qed.
-
-
-  (* Lemma reach_res_approx (S : Ensemble loc) (H1 H2 : heap block) *)
-  (*       (v : value) (n : nat) : *)
-  (*   (reach' H1 S) |- H1 ≡ H2  -> *)
-  (*   (val_loc v) \in S ->  *)
-  (*   res_approx_fuel n (v, H1) (v, H2). *)
-  (* Proof. *)
-  (*   intros Hsub Hin . *)
-  (*   assert (Hr : reach' H1 S <--> reach' H2 S). *)
-  (*   { eapply reach'_heap_eq. eauto. } *)
-  (*   revert H1 H2 S v Hr Hsub Hin. *)
-  (*   induction n using lt_wf_rec1; intros H1 H2 S v Hr Hsub Hin. *)
-  (*   destruct n; destruct v. *)
-  (*   - rewrite res_approx_fuel_eq. intros c vs Hget. *)
-  (*     rewrite Hsub in Hget. eexists; split; eauto. intros; omega. *)
-  (*     eapply reach'_extensive. eassumption. *)
-  (*   - rewrite res_approx_fuel_eq; split; [ reflexivity |]; intros rho B Hget. *)
-  (*     rewrite Hsub in Hget. *)
-  (*     eexists; split; eauto. intros; omega. now eapply reach'_extensive. *)
-  (*   - rewrite res_approx_fuel_eq. intros c vs Hget. *)
-  (*     assert (Hget1 := Hget). *)
-  (*     rewrite Hsub in Hget; [| now eapply reach'_extensive ]. *)
-  (*     eexists; split; eauto. intros i Hlt. *)
-  (*     eapply Forall2_same.  intros l' Hin'. *)
-  (*     eapply H with (S := Union _ S (post H1 S)); eauto. *)
-  (*     rewrite <- reach_spec with (H := H1) (S := S). *)
-  (*     rewrite <- reach_spec with (H := H2) (S := S). *)
-  (*     eassumption. now eauto with Ensembles_DB. *)
-  (*     apply Union_Included. now apply reach'_extensive. *)
-  (*     eapply Included_trans with (s2 := post H2 S). *)
-  (*     eapply (heap_eq_antimon) in Hsub; [| now apply reach'_extensive ]. *)
-  (*     rewrite post_heap_eq; eauto. reflexivity. *)
-  (*     now apply Included_post_reach'. *)
-  (*     now eauto with Ensembles_DB. *)
-  (*     apply Union_Included. now apply reach'_extensive. *)
-  (*     eapply Included_trans with (s2 := post H2 S). *)
-  (*     eapply (heap_eq_antimon) in Hsub; [| now apply reach'_extensive ]. *)
-  (*     rewrite post_heap_eq; eauto. reflexivity. *)
-  (*     rewrite Hr. now apply Included_post_reach'. *)
-  (*     now rewrite <- reach'_post. *)
-  (*     right. exists l. eexists. repeat split; eauto. *)
-  (*     unfold locs. rewrite FromList_map_image_FromList. eexists. *)
-  (*     split; eauto. *)
-  (*   - rewrite res_approx_fuel_eq; split; [ reflexivity |]; intros rho B Hget. *)
-  (*     assert (Hget1 := Hget). *)
-  (*     rewrite Hsub in Hget; [| now apply reach'_extensive ]. *)
-  (*     eexists; split; eauto. intros i x Hlt Hin'. *)
-  (*     destruct (M.get x rho) eqn:Heq. *)
-  (*     * left; do 2 eexists. split; [| split ]; eauto. *)
-  (*       eapply H with (S := Union _ S (post H1 S)); eauto. *)
-  (*       rewrite <- reach_spec with (H := H1) (S := S). *)
-  (*       rewrite <- reach_spec with (H := H2) (S := S). *)
-  (*       eassumption. now eauto with Ensembles_DB. *)
-  (*       apply Union_Included. now apply reach'_extensive. *)
-  (*       eapply Included_trans with (s2 := post H2 S). *)
-  (*       eapply (heap_eq_antimon) in Hsub; [| now apply reach'_extensive ]. *)
-  (*       rewrite post_heap_eq; eauto. reflexivity. *)
-  (*       now apply Included_post_reach'. *)
-  (*       now eauto with Ensembles_DB. *)
-  (*       apply Union_Included. now apply reach'_extensive. *)
-  (*       eapply Included_trans  with (s2 := post H2 S). *)
-  (*       eapply (heap_eq_antimon) in Hsub; [| now apply reach'_extensive ]. *)
-  (*       rewrite post_heap_eq; eauto. reflexivity. *)
-  (*       rewrite Hr. now apply Included_post_reach'. *)
-  (*       now rewrite <- reach'_post. *)
-  (*       right. exists l. eexists. repeat split; eauto. *)
-  (*       exists x. split; eauto. rewrite Heq. reflexivity. *)
-  (*     * right; eauto. *)
-  (* Qed. *)
-  
-  (* Corollary reach_res_equiv (S : Ensemble loc) (H1 H2 : heap block) *)
-  (*           (v : value) : *)
-  (*   (reach' H1 S) |- H1 ≡ H2 -> *)
-  (*   val_loc v \in S ->  *)
-  (*   (v, H1) ≈ (v, H2). *)
-  (* Proof. *)
-  (*   intros Hsub Hin n; split; rewrite <- res_approx_fuel_eq; *)
-  (*   eapply reach_res_approx; eauto. rewrite <- reach'_heap_eq. *)
-  (*   symmetry. eassumption. eassumption. *)
-  (* Qed. *)
-  
-  Lemma Preorder_res_equiv_fuel i : preorder res (res_approx_fuel i).
-  Proof.
-    constructor.
-    - induction i as [i IHi] using lt_wf_rec.
-      intros [v H1]. rewrite res_approx_fuel_eq. destruct v.
-      simpl. destruct (get l H1) eqn:Hgetl; eauto. 
-      destruct b as [c vs | rho B f]. 
-      + eexists; split; eauto.
-        intros i' Hlt.
-        eapply Forall2_refl; intros l'. eapply IHi. eassumption.
-      + eexists; split; eauto. 
-        intros x.
-        destruct (M.get x rho) eqn:heq; eauto.
-        * left. do 2 eexists; repeat split; eauto.
-          intros. eapply IHi; eauto.
-      + split; eauto.
-    - induction i as [i IHi]  using lt_wf_rec1.
-      intros [v1 H1] [v2 H2] [v3 H3] Hap1 Hap2. rewrite res_approx_fuel_eq in *.
-      simpl in *.
-      destruct v1 as [l1 | B1 f1]; destruct v2 as [l2 | B2 f2]; destruct v3 as [l3 | B3 f3];
-      try contradiction.
-      { destruct (get l1 H1) eqn:Hget1; eauto.
-        destruct b as [c vs1 | rho1 B f].
-        + edestruct Hap1 as [vs2 [Hget2 Hall2]]. rewrite Hget2 in Hap2.
-          destruct Hap2 as [vs3 [Hget3 Hall3]].
-          eexists; split; eauto.
-          intros i' Hlt.
-          eapply Forall2_trans_strong; eauto. intros v1 v2 v3 Hv1 Hv2.
-          eapply IHi. eassumption. simpl in Hv1. eassumption.
-          simpl in Hv2. eassumption.
-        + edestruct Hap1 as [rho2 [Hget2 Hall2]]. rewrite Hget2 in Hap2.
-          destruct Hap2 as [rho33 [Hget3 Hall3]].
-          eexists; split; eauto.
-          intros x.
-          edestruct Hall2 as [[l1' [l2' [Hgetl1 [Hgetl2 Hi]]]] | [Hn1 Hn2]]; eauto.
-          * edestruct Hall3 as [[l2'' [l3' [Hgetl2' [Hgetl3 Hi']]]] | [Hn1 Hn2]]; eauto.
-            repeat subst_exp.
-            left; repeat eexists; eauto. subst_exp.
-            intros. eapply IHi; eauto.
-            congruence.
-          * edestruct Hall3 as [[l2'' [l3' [Hgetl2' [Hgetl3 Hi']]]] | [Hn2' Hn3]]; eauto.
-            congruence. }
-      { inv Hap1; inv Hap2. split; eauto. }
-  Qed.
-  
-  Instance Reflexive_res_equiv_fuel i : Reflexive (res_approx_fuel i).
-  Proof.
-    eapply Preorder_res_equiv_fuel.
-  Qed.
-
-  Instance Transitive_res_equiv_fuel i : Transitive (res_approx_fuel i).
-  Proof.
-    eapply Preorder_res_equiv_fuel.
-  Qed.
-
-  Instance Equivalence_res_equiv : Equivalence res_equiv.
-  Proof.
-    constructor. 
-    - intros res; split; eapply Preorder_res_equiv_fuel.
-    - intros res res' H n. destruct (H n) as [H1 H2]. split; eauto.
-    - intros res1 res2 res3 H1 H2. intros n.
-      destruct (H1 n) as [Ht1 Ht2]; destruct (H2 n) as [Ht3 Ht4];
-      split.
-      now eapply Preorder_res_equiv_fuel; eauto.
-      now eapply Preorder_res_equiv_fuel; eauto.
-  Qed.
-
-  Instance Equivalence_heap_env_equiv S : Equivalence (heap_env_equiv S).
-  Proof.
-    constructor.
-    - intros [H rho]; split; intros l Hget; eexists; split; eauto; reflexivity.
-    - intros [H rho] [H' rho'] H1; split; intros v l Hin Hget;
-      eapply H1; eauto.
-    - edestruct Equivalence_res_equiv; eauto.
-      intros [H rho] [H' rho'] [H'' rho''] H1 H2; split; intros v l Hin Hget.
-      edestruct H1 as [H1' _]; eauto. edestruct H1' as [v1 [Hget1 Hres1]]; eauto.
-      edestruct H2 as [H2' _]; eauto. edestruct H2' as [v2 [Hget2 Hres2]]; eauto.
-      edestruct H2 as [_ H2']; eauto. edestruct H2' as [v2 [Hget2 Hres2]]; eauto.
-      edestruct H1 as [_ H1']; eauto. edestruct H1' as [v1 [Hget1 Hres1]]; eauto.
-  Qed.
-
-  (** * Lemmas about [block_equiv] **)
-  
-  Instance Reflexive_block_equiv : Reflexive block_equiv.
-  Proof.
-    intros [H b]. destruct b; simpl; eauto; try reflexivity.
-    split; eauto. eapply Forall2_refl; now eauto with typeclass_instances.
-  Qed.
-  
-  Instance Transitive_block_equiv : Transitive block_equiv.
-  Proof.
-    intros [H1 b1] [H2 b2] [H3 b3] Hb1 Hb2.
-    destruct b1; destruct b2; try contradiction;
-    destruct b3; try contradiction.
-    - destruct Hb1 as [Heq1 Hb1].
-      destruct Hb2 as [Heq2 Hb2].
-      subst. split; eauto. 
-      eapply Forall2_trans_strong; try eassumption.
-      simpl; intros. eapply Equivalence_Transitive; eauto. 
-    - simpl in *.
-      eapply Equivalence_Transitive; eauto.
-  Qed.
-  
-  Instance Symmetric_block_equiv : Symmetric block_equiv.
-  Proof.
-    intros [H1 b1] [H2 b2] Hb.
-    destruct b1; destruct b2; try contradiction.
-    - destruct Hb as [Heq1 Hb1].
-      subst. split; eauto. 
-      eapply Forall2_symm_strong; try eassumption.
-      simpl; intros. symmetry. eauto.
-    - simpl in *. symmetry; eauto.
-  Qed.
-
-  Instance Equivalence_heap_equiv S : Equivalence (heap_equiv S). 
-  Proof.
-    constructor.
-    - intros H.
-      split; intros x l Hin Hget;
-      eexists; split; eauto; reflexivity.
-    - intros H1 H2 [Hs1 Hs2].
-      split; intros x l Hin Hget. 
-      edestruct (Hs2 x l Hin Hget) as [b1 [Hget1 Heq1]]. 
-      eexists; split; eauto; symmetry; eauto.
-      edestruct (Hs1 x l Hin Hget) as [b1 [Hget1 Heq1]]. 
-      eexists; split; eauto; symmetry; eauto.
-    - intros H1 H2 H3 [Hs1 Hs2] [Hs2' Hs3].
-      split; intros x l Hin Hget. 
-      edestruct (Hs1 x l Hin Hget) as [b1 [Hget1 Heq1]]. 
-      edestruct (Hs2' _ _ Hin Hget1) as [b2 [Hget2 Heq2]].
-      eexists; split; eauto. now eapply Transitive_block_equiv; eauto.
-      edestruct (Hs3 x l Hin Hget) as [b1 [Hget1 Heq1]]. 
-      edestruct (Hs2 _ _ Hin Hget1) as [b2 [Hget2 Heq2]].
-      eexists; split; eauto. eapply Transitive_block_equiv; eauto.
-  Qed.
-      
-  (** [heap_env_approx] and [heap_env_equiv] equivalence properties *)
-  Lemma reach_approx (S : Ensemble var) (H1 H2 : heap block) (rho : env) : 
-    (env_locs rho S) |- H1 ≃ H2 -> 
-    heap_env_approx S (H2, rho) (H1, rho).
-  Proof.
-    intros [Heq1 Heq2] x v Hin Hget.
-    eexists; split; eauto.  
-    rewrite res_equiv_eq. simpl.
-    destruct v as [l | B f]; [| now split; eauto ].
-    destruct (get l H1) eqn:Heq.
-    - eapply Heq1 in Heq.
-      destruct Heq as [b2 [Hb2 Heqb]]. rewrite Hb2.
-      simpl in Heqb. destruct b; destruct b2; try contradiction.
-      destruct Heqb as [Heqc Hall]; subst; split; eauto.
-      eapply Forall2_symm_strong; eauto.
-      simpl; intros.
-      now eapply Equivalence.equiv_symmetric; eauto.
-      now symmetry; eauto. eapply get_In_env_locs; eauto.
-      reflexivity.
-    - destruct (get l H2) eqn:HgetH2; eauto.
-      eapply Heq2 in HgetH2.
-      destruct HgetH2 as [b2 [Hgetb2 _]].
-      congruence.
-      eexists; split; eauto. rewrite Hget; eauto. reflexivity.
-  Qed.   
-
-  Corollary reach_heap_env_equiv (S : Ensemble var) (H1 H2 : heap block)
-            (rho : env) :
-    (env_locs rho S) |- H1 ≃ H2 -> 
-    S |- (H1, rho) ⩪ (H2, rho).
-  Proof.
-    intros. split; eapply reach_approx; simpl; try eassumption.
-    symmetry. eassumption.
-  Qed.
-
-  Lemma heap_equiv_res_equiv (S : Ensemble loc) (H1 H2 : heap block)
-        (v : value) :
-    S |- H1 ≃ H2  ->
-    (val_loc v) \subset S -> 
-    (v, H1) ≈ (v, H2).
-  Proof.
-    intros Heq Hin m.
-    split. eapply heap_equiv_res_approx; eauto. 
-    eapply heap_equiv_res_approx; eauto. symmetry.
-    eassumption. 
-  Qed.
-  
-  (** Proper instances *)
-
-  Instance Proper_heap_env_approx : Proper (Same_set _ ==> eq ==> eq ==> iff) heap_env_approx.
-  Proof.
-    intros s1 s2 hseq p1 p2 Heq p1' p2' Heq'; subst; split; intros H1;
-    destruct p2; destruct p2'; firstorder.
-  Qed.
-
-  Instance Proper_heap_env_equiv : Proper (Same_set _ ==> eq ==> eq ==> iff) heap_env_equiv.
-  Proof.
-    intros s1 s2 hseq p1 p2 Heq p1' p2' Heq'; subst.
-    split; intros [h1 h2]; split; (try now rewrite hseq; eauto);
-    rewrite <- hseq; eauto.
-  Qed.
-
-  Instance Proper_heap_equiv : Proper (Same_set _ ==> eq ==> eq ==> iff) heap_equiv.
-  Proof.
-    intros s1 s2 hseq p1 p2 Heq p1' p2' Heq'; subst.
-    split; intros [h1 h2].
-    split; intros b l HIn; eauto; [eapply h1 | eapply h2]; eapply hseq; eassumption.
-    split; intros b l HIn; eauto; [eapply h1 | eapply h2]; eapply hseq; eassumption.
-  Qed.
-  
-  (** Monotonicity properties *)
-
-  Lemma heap_env_equiv_antimon S1 S2 H1 H2 rho1 rho2 :
-    S1 |- (H1, rho1) ⩪ (H2, rho2) ->
-    S2 \subset S1 ->
-    S2 |- (H1, rho1) ⩪ (H2, rho2).
-  Proof.
-    firstorder.
-  Qed.
-
-  (** Weakening lemmas *)
-
-  (* TODO move *)
-  Lemma In_Union_list {A} (l : list (Ensemble A)) s:
-    List.In s l ->
-    s \subset Union_list l.
-  Proof.
-    intros Hin. induction l. 
-    - now inv Hin.
-    - inv Hin. now eapply Included_Union_l.
-      simpl. eapply Included_Union_preserv_r.
-      eapply IHl; eauto.
-  Qed.
-
-      
-  Lemma res_approx_weakening (S1 S2 : Ensemble loc) (H1 H2 H1' H2' : heap block)
-        (v1 v2 : value) (i : nat) :
-    closed S1 H1 -> closed S2 H2 ->
-    res_approx_fuel' i (v1, H1) (v2, H2) ->
-    H1 ⊑ H1' -> 
-    H2 ⊑ H2' ->
-    val_loc v1 \subset S1 -> val_loc v2 \subset S2 -> 
-    res_approx_fuel' i (v1, H1') (v2, H2').
-  Proof.
-    intros Hwf1 Hwf2 Heq Hsub1 Hsub2.
-    revert v1 v2 Heq; induction i using lt_wf_rec1;
-    intros v1 v2 Heq Hdom1 Hdom2.
-    destruct v1 as [ l1 | B1 f1]; destruct v2 as [ l2 | V2 f2]; try contradiction. 
-    { edestruct Hwf1 as [b1 [Hget1 Hsub1']].
-      eapply Hdom1; reflexivity. 
-      edestruct Hwf2 as [b2 [Hget2 Hsub2']].
-      eapply Hdom2; reflexivity. 
-      specialize (Hsub1 _ _ Hget1).
-      specialize (Hsub2 _ _ Hget2).
-      simpl in Hget1, Hget2, Hsub1, Heq. 
-      simpl.
-      rewrite Hsub1. rewrite Hget1 in Heq. destruct b1.
-      - edestruct Heq as [vs2 [Hgetl2 Hall]]; eauto.
-        subst_exp.
-      eexists; split; [ now eauto |].
-      intros i' Hlt.
-      eapply Forall2_monotonic_strong
-      with (R :=
-              fun l3 l4 =>
-                val_loc l3 \subset S1 ->
-                val_loc l4 \subset S2 -> res_approx_fuel i' (l3, H1) (l4, H2)).
-      * intros v1' v2' Hin1 Hin2 Hyp. 
-        rewrite res_approx_fuel_eq. eapply H; eauto.
-        rewrite <- res_approx_fuel_eq. eapply Hyp; eauto.
-        simpl in Hsub1'. eapply Included_trans; [| eassumption].
-        eapply In_Union_list. now eapply in_map; eauto.
-        simpl in Hsub2'. eapply Included_trans; [| eassumption].
-        eapply In_Union_list. now eapply in_map; eauto.
-        simpl in Hsub1'. eapply Included_trans; [| eassumption].
-        eapply In_Union_list. now eapply in_map; eauto.
-        simpl in Hsub2'. eapply Included_trans; [| eassumption].
-        eapply In_Union_list. now eapply in_map; eauto.
-      * eapply Forall2_monotonic; [| eauto ].
-        intros. eassumption.
-    - edestruct Heq as [rho2 [Hgetl2 Hall]]; eauto.
-      subst_exp.
-      eexists; split; [ now eauto |].
-      intros x.
-      edestruct Hall as [[v1 [v2 [Hs1 [Hs2 Hi]]]] | Hnone]; eauto.
-      left. repeat eexists; eauto. intros i' Hlt.
-      rewrite res_approx_fuel_eq. eapply H; eauto.
-      rewrite <- res_approx_fuel_eq. eapply Hi. eassumption.
-      simpl in Hsub1'. eapply Included_trans; [| eassumption].
-      eapply get_In_env_locs; eauto. now constructor.
-      simpl in Hsub2'. eapply Included_trans; [| eassumption].
-      eapply get_In_env_locs; eauto. now constructor. }
-    { simpl in *; eassumption. }
-  Qed.
-  
-  Corollary res_equiv_weakening (S1 S2 : Ensemble loc) (H1 H2 H1' H2' : heap block)
-            (v1 v2 : value) :
-    closed S1 H1 -> closed S2 H2 ->
-    (v1, H1) ≈ (v2, H2) ->
-    H1 ⊑ H1' ->
-    H2 ⊑ H2' ->
-    val_loc v1 \subset S1 -> val_loc v2 \subset S2 -> 
-    (v1, H1') ≈ (v2, H2').
-  Proof.
-    intros Hwf1 Hwf2 Heq Hsub1 Hsub2 Hin1 Hin2 n. destruct (Heq n) as [Heq1 He2].
-    split; rewrite res_approx_fuel_eq.
-    eapply (res_approx_weakening S1 S2 H1 H2 H1' H2'); eauto.
-    now rewrite <- res_approx_fuel_eq.
-    eapply (res_approx_weakening S2 S1 H2 H1 H2' H1'); eauto.
-    now rewrite <- res_approx_fuel_eq. 
-  Qed.
-
-
-  Lemma heap_env_approx_weakening S H1 H2 H1' H2' rho1 rho2 :
-    well_formed (reach' H1 (env_locs rho1 S)) H1 ->
-    well_formed (reach' H2 (env_locs rho2 S)) H2 ->
-    env_locs rho1 S \subset dom H1 ->
-    env_locs rho2 S \subset dom H2 ->
-    S |- (H1, rho1) ⩪ (H2, rho2) ->
-    H1 ⊑ H1' ->
-    H2 ⊑ H2' ->
-    heap_env_approx S (H1', rho1) (H2', rho2).
-  Proof.
-    intros Hwf1 Hwf2 He1 He2  [Heq1 Heq2] Hal1 Hal2 y l Hin Hget; simpl.
-    edestruct Heq1 as [x' [Hget' Heq']]; eauto.
-    eexists; split; eauto.
-    eapply (res_equiv_weakening _ _ H1 H2).
-    eapply reach'_closed. now apply Hwf1. eassumption.
-    eapply reach'_closed. now apply Hwf2. eassumption.
-    eassumption. eassumption. eassumption.
-    eapply Included_trans; [| eapply reach'_extensive ].
-    now eapply get_In_env_locs; eauto.
-    eapply Included_trans; [| eapply reach'_extensive ].
-    now eapply get_In_env_locs; eauto.
-  Qed.
-  
-  Corollary heap_env_equiv_weaking_cor S H1 H2 H1' H2' rho1 rho2 :
-    well_formed (reach' H1 (env_locs rho1 S)) H1 ->
-    well_formed (reach' H2 (env_locs rho2 S)) H2 ->
-    env_locs rho1 S \subset dom H1 ->
-    env_locs rho2 S \subset dom H2 ->
-    S |- (H1, rho1) ⩪ (H2, rho2) ->
-    H1 ⊑ H1' ->
-    H2 ⊑ H2' ->
-    S |- (H1', rho1) ⩪ (H2', rho2).
-  Proof.
-    intros. split.
-    now eapply (heap_env_approx_weakening _ H1 H2); eauto.
-    now eapply (heap_env_approx_weakening _ H2 H1); eauto; symmetry.
-  Qed.
-
-  Lemma heap_env_approx_weakening' S S1 S2 H1 H2 H1' H2' rho1 rho2 :
-     closed S1 H1 -> closed S2 H2 ->
-     env_locs rho1 S \subset S1 ->
-     env_locs rho2 S \subset S2 ->
-     S |- (H1, rho1) ⩪ (H2, rho2) ->
-     H1 ⊑ H1' ->
-     H2 ⊑ H2' ->
-     heap_env_approx S (H1', rho1) (H2', rho2).
-   Proof.
-     intros Hwf1 Hwf2 He1 He2  [Heq1 Heq2] Hal1 Hal2 y l Hin Hget; simpl.
-     edestruct Heq1 as [x' [Hget' Heq']]; eauto.
-     eexists; split; eauto.
-     eapply (res_equiv_weakening _ _ H1 H2); eauto.
-     eapply Included_trans; [| eassumption ].
-     now eapply get_In_env_locs; eauto.
-     eapply Included_trans; [| eassumption ].
-     now eapply get_In_env_locs; eauto.
-   Qed.
-   
-   Corollary heap_env_equiv_weaking' S S1 S2 H1 H2 H1' H2' rho1 rho2 :
-     closed S1 H1 -> closed S2 H2 ->
-     env_locs rho1 S \subset S1 ->
-     env_locs rho2 S \subset S2 ->
-     S |- (H1, rho1) ⩪ (H2, rho2) ->
-     H1 ⊑ H1' ->
-     H2 ⊑ H2' ->
-     S |- (H1', rho1) ⩪ (H2', rho2).
-   Proof.
-     intros. split.
-     now eapply (heap_env_approx_weakening' _ _ _ H1 H2); eauto.
-     now eapply (heap_env_approx_weakening' _ _ _ H2 H1); eauto; symmetry.
-   Qed.
-  
-  (** [heap_env_approx] and [heap_env_equiv] preservation under store and heap extension *)
-   
-  Lemma heap_env_approx_set S H1 H2 x l1 l2 rho1 rho2 :
-    heap_env_approx (Setminus _ S (Singleton _ x)) (H1, rho1) (H2, rho2) ->
-    (l1, H1) ≈ (l2, H2) ->
-    heap_env_approx S (H1, M.set x l1 rho1) (H2, M.set x l2 rho2).
-  Proof.
-    intros Heq Hreq. intros y l Hin Hget.
-    destruct (peq x y); subst; simpl in *. 
-    - exists l2. rewrite M.gss in *; inv Hget; eauto.
-    - rewrite M.gso in *; eauto. eapply Heq in Hget; eauto.
-      constructor; eauto. intros Hc; inv Hc; congruence.
-  Qed.
-
-  Lemma heap_env_equiv_set S H1 H2 x l1 l2 rho1 rho2 :
-    Setminus _ S (Singleton _ x) |- (H1, rho1) ⩪ (H2, rho2) ->
-    (l1, H1) ≈ (l2, H2) ->
-    S  |- (H1, M.set x l1 rho1) ⩪ (H2, M.set x l2 rho2).
-  Proof.
-    intros [Heq1 Heq2] Hreq. split.
-    now eapply heap_env_approx_set.
-    now eapply heap_env_approx_set; eauto; symmetry.
-  Qed.
-
-  Lemma heap_env_equiv_setlist S H1 H2 xs ls1 ls2 rho1 rho2 rho1' rho2' :
-    Setminus _ S (FromList xs) |- (H1, rho1) ⩪ (H2, rho2) ->
-    setlist xs ls1 rho1 = Some rho1' -> setlist xs ls2 rho2 = Some rho2' ->
-    Forall2 (fun l1 l2 => (l1, H1) ≈ (l2, H2)) ls1 ls2  ->
-    S |- (H1, rho1') ⩪ (H2, rho2').
-  Proof with (now eauto with Ensembles_DB).
-    revert S rho1' rho2' ls1 ls2; induction xs;
-    intros S  rho1' rho2' ls1 ls2 Heq Hs1 Hs2 Hall.
-    - destruct ls1; destruct ls2; try discriminate. inv Hs1; inv Hs2; eauto.
-      rewrite FromList_nil, Setminus_Empty_set_neut_r in Heq. eassumption.
-    - destruct ls1; destruct ls2; try discriminate.
-      inv Hall. simpl in Hs1, Hs2.
-      destruct (setlist xs ls1 rho1) eqn:Hset1; try discriminate.
-      destruct (setlist xs ls2 rho2) eqn:Hset2; try discriminate.
-      inv Hs1; inv Hs2. eapply heap_env_equiv_set; eauto.
-      eapply IHxs; eauto. eapply heap_env_equiv_antimon; eauto.
-      rewrite FromList_cons...
-  Qed.
-  
-
-  Lemma heap_env_approx_alloc S S1 S2 H1 H2 H1' H2' rho1 rho2 l1 l2 b1 b2 x :
-    closed S1 H1 -> closed S2 H2 ->
-    env_locs rho1 (S \\ [set x]) \subset S1 ->
-    env_locs rho2 (S \\ [set x]) \subset S2 ->
-    locs b1 \subset S1 -> locs b2 \subset S2 ->
-    S \\ [set x] |- (H1, rho1) ⩪ (H2, rho2) ->
-    alloc b1 H1 = (l1, H1') -> 
-    alloc b2 H2 = (l2, H2') ->
-    block_equiv (H1, b1) (H2, b2) ->
-    heap_env_approx S (H1', M.set x (Loc l1) rho1) (H2', M.set x (Loc l2) rho2).
-  Proof.
-    intros Hc1 Hc2 Hsub1 Hsub2 Hin1 Hin2 Heq Ha1 Ha2 Hb y v1 Hin Hget.
-    destruct (peq x y); subst.
-    - rewrite M.gss in Hget. inv Hget.
-      eexists; split. rewrite M.gss. reflexivity.
-      rewrite res_equiv_eq. simpl.
-      erewrite gas; eauto. erewrite gas; eauto.
-      simpl in Hb. destruct b1; destruct b2; try contradiction.
-      + destruct Hb as [Heq' Hall]; subst.
-        split; eauto.
-        eapply Forall2_monotonic_strong; eauto.
-        intros. 
-        eapply res_equiv_weakening. exact Hc1. exact Hc2.
-        eassumption.
-        now eapply alloc_subheap; eauto.
-        now eapply alloc_subheap; eauto.
-        eapply Included_trans; [| eassumption ].
-        eapply In_Union_list. now eapply in_map; eauto.
-        eapply Included_trans; [| eassumption ].
-        eapply In_Union_list. now eapply in_map; eauto.
-      + eapply heap_env_equiv_weaking'.
-        exact Hc1. exact Hc2.
-        eassumption. eassumption. eassumption.
-        now eapply alloc_subheap; eauto.
-        now eapply alloc_subheap; eauto.
-    - rewrite M.gso in Hget; eauto.
-      destruct Heq as [Heq1 Heq2].
-      edestruct Heq1 as [v2 [Hget2 Hb']]; eauto.
-      constructor; eauto. now intros Hc; inv Hc; eauto.
-      eexists.
-      rewrite M.gso; eauto. split; eauto.
-      eapply res_equiv_weakening. exact Hc1. exact Hc2.
-      eassumption.
-      now eapply alloc_subheap; eauto.
-      now eapply alloc_subheap; eauto.
-      eapply Included_trans; [| now apply Hsub1 ].
-      eapply get_In_env_locs; eauto.
-      constructor; eauto. now intros Hc; inv Hc; eauto.
-      eapply Included_trans; [| now apply Hsub2 ].
-      eapply get_In_env_locs; eauto.
-      constructor; eauto. now intros Hc; inv Hc; eauto.      
-  Qed.
-  
-  Corollary heap_env_equiv_alloc S S1 S2 H1 H2 H1' H2' rho1 rho2 l1 l2 b1 b2 x :
-    closed S1 H1 -> closed S2 H2 ->
-    env_locs rho1 (S \\ [set x]) \subset S1 ->
-    env_locs rho2 (S \\ [set x]) \subset S2 ->
-    locs b1 \subset S1 -> locs b2 \subset S2 ->
-    S \\ [set x] |- (H1, rho1) ⩪ (H2, rho2) ->
-    alloc b1 H1 = (l1, H1') -> 
-    alloc b2 H2 = (l2, H2') ->
-    block_equiv (H1, b1) (H2, b2) ->
-    S |- (H1', M.set x (Loc l1) rho1) ⩪ (H2', M.set x (Loc l2) rho2).
-  Proof.
-    intros. split. now eapply (heap_env_approx_alloc S S1 S2); eauto.
-    eapply (heap_env_approx_alloc S S2 S1); eauto; symmetry; eassumption.
-  Qed.
-
-  Lemma def_funs_subheap H H' rho rho' B B0 c l :
-    (H', rho') = def_closures B B0 rho H c l ->
-    H ⊑ H'.
-  Proof.
-    revert H' rho'; induction B; intros H' rho' Heq;
-    simpl; [| inv Heq; now apply subheap_refl ].
-    simpl in Heq. destruct (def_closures B B0 rho H c l) as [H'' rho''].
-    destruct (alloc _ H'') as [l' H'''] eqn:Heq'.
-    inv Heq. eapply subheap_trans; eauto.
-    now eapply alloc_subheap; eauto.
-  Qed.
-  
-  Lemma closed_alloc' S H H' l v :
-    closed S H ->
-    locs v \subset S ->
-    alloc v H = (l, H') ->
-    closed S H'.
+  Lemma closed_set_alloc_alt S H H' b l rho x :
+    closed (reach' H (env_locs rho (S \\ [set x]))) H ->
+    locs b \subset (reach' H (env_locs rho (S \\ [set x]))) ->
+    alloc b H = (l, H') ->
+    closed (reach' H' (env_locs (M.set x (Loc l) rho) S)) H'.
   Proof with now eauto with Ensembles_DB.
     intros Hcl Hin Ha l1 Hin'.
     destruct (loc_dec l1 l); subst.
     - eexists. erewrite gas; eauto.
-    - edestruct Hcl as [l2 [Hget Hsub]]; try eassumption.
-      eexists. erewrite gao; eauto; split; eauto.
-  Qed.
+      split. reflexivity.
+      eapply Included_trans. eassumption.
+      eapply Included_trans.
+      eapply reach'_heap_monotonic.
+      now eapply alloc_subheap; eauto.
+      eapply reach'_set_monotonic.
+      rewrite <- env_locs_set_not_In.
+      eapply env_locs_monotonic...
+      intros Hinx. now inv Hinx; eauto.
+    - eapply reach'_set_monotonic in Hin';
+      [| now eapply env_locs_set_Inlcuded'].
+      rewrite reach'_Union in Hin'.
+      rewrite reach_unfold in Hin'.
+      simpl in Hin'. rewrite post_Singleton in Hin'; [| now erewrite gas; eauto ].
+      inv Hin'.
+      + inv H0.
+        * inv H1. congruence.
+        * edestruct Hcl as [b1 [Hget1 Hsub]]; eauto.
+          rewrite <- reach'_alloc; try eassumption.
+          rewrite reach'_idempotent.
+          eapply reach'_set_monotonic; [| eassumption ].
+          eapply Included_trans. eassumption.
+          eapply reach'_heap_monotonic.
+          eapply alloc_subheap. eassumption.
+          eexists; split; eauto.
+          
+          now erewrite gao; eauto.
+          
+          eapply Included_trans. eassumption.
+          eapply Included_trans. eapply reach'_heap_monotonic.
+          eapply alloc_subheap. eassumption.
+          eapply reach'_set_monotonic. 
+          rewrite <- env_locs_set_not_In.
+          eapply env_locs_monotonic...
+          intros Hc. inv Hc; eauto.            
+      + edestruct Hcl as [b1 [Hget1 Hsub]]; eauto.
+        rewrite <- reach'_alloc; try eassumption.
+        eexists.
+        erewrite gao; eauto; split; eauto.
+        eapply Included_trans. eassumption.
+        eapply Included_trans. eapply reach'_heap_monotonic.
+        eapply alloc_subheap. eassumption.
+        eapply reach'_set_monotonic. 
+        rewrite <- env_locs_set_not_In.
+        eapply env_locs_monotonic...
+        intros Hc. inv Hc; eauto.
+  Qed.  
 
-  Lemma closed_alloc_Union S H H' l v :
-    closed S H ->
-    locs v \subset S ->
-    alloc v H = (l, H') ->
-    closed (l |: S) H'.
-  Proof with now eauto with Ensembles_DB.
-    intros Hcl Hin Ha l1 Hin'.
-    destruct (loc_dec l1 l); subst.
-    - eexists. erewrite gas; eauto. split; eauto...
-    - inv Hin'. inv H0. contradiction.
-      edestruct Hcl as [l2 [Hget Hsub]]; try eassumption.
-      eexists. erewrite gao; eauto; split; eauto...
-  Qed.
-
-  Lemma closed_def_funs S1 H1 H1' rho1 rho1'  B B0 c l :
-    closed S1 H1 ->
-    l \in S1 ->
-    (H1', rho1') = def_closures B B0 rho1 H1 c l ->
-    closed S1 H1'.
+  (* TODO move *)
+  Lemma Forall2_nthN' (A B : Type) (R : A -> B -> Prop) (l1 : list A) 
+        (l2 : list B) (n : N) (v1 : A) (v2 : B):
+    Forall2 R l1 l2 ->
+    nthN l1 n = Some v1 ->
+    nthN l2 n = Some v2 ->
+    R v1 v2.
   Proof.
-    revert H1' rho1'; induction B;
-    intros H1' rho1' Hc Hsub Heq; [| inv Heq; now eauto ].
-    simpl in Heq. destruct (def_closures B B0 rho1 H1 c l) as [H'' rho''].
-    destruct (alloc _ H'') as [l' H'''] eqn:Heq'.
-    inv Heq. eapply closed_alloc'; [| | eassumption ]; eauto.
-    simpl. rewrite Union_Empty_set_neut_r, Union_Empty_set_neut_l.
-    eapply Singleton_Included. eassumption.
-  Qed.
-
-  Lemma env_locs_def_funs S S1 H1 H1' rho1 rho1'  B B0 c l :
-    env_locs rho1 (Setminus _ S (name_in_fundefs B)) \subset S1 ->
-    l \in S1 ->
-    (H1', rho1') = def_closures B B0 rho1 H1 c l ->
-    env_locs rho1' (Setminus _ S (name_in_fundefs B)) \subset S1.
-  Proof.
-    revert S H1' rho1'; induction B; intros S H1' rho1' Hsub1 Hsub2 Heq.
-    - simpl in Heq. destruct (def_closures B B0 rho1 H1 c l) as [H'' rho''].
-      destruct (alloc _ H'') as [l' H'''] eqn:Heq'.
-      inv Heq. rewrite env_locs_set_not_In.
-      simpl; rewrite <- !Setminus_Union.
-      simpl in Hsub1; rewrite <- !Setminus_Union in Hsub1.
-      eapply IHB; eauto.
-      intros Hc. inversion Hc as [Hc1 Hc2]; eauto. 
-      eapply Hc2; left; eauto.
-    - simpl in Hsub1.
-      rewrite Setminus_Empty_set_neut_r in Hsub1; inv Heq.
-      rewrite Setminus_Empty_set_neut_r; eauto.
-  Qed.
-
-  Lemma def_funs_exists_new_set S S1 H1 H1' rho1 rho1' B B0 c l :
-    closed S1 H1 ->
-    env_locs rho1 (Setminus _ S (name_in_fundefs B)) \subset S1 ->
-    l \in S1 ->
-    (H1', rho1') = def_closures B B0 rho1 H1 c l ->
-    exists S1', S1 \subset S1' /\ closed S1' H1' /\
-           env_locs rho1' S \subset S1'.
-  Proof with now eauto with Ensembles_DB.
-    revert S H1' rho1'; induction B; intros S H1' rho1' Hc Hsub1 Hsub2 Heq.
-    - simpl in Heq. destruct (def_closures B B0 rho1 H1 c l) as [H'' rho''].
-      destruct (alloc _ H'') as [l' H'''] eqn:Heq'.
-      inv Heq.
-      edestruct IHB as [S1' [Hsub [Hc' Henv]]]; eauto.
-      eapply Included_trans; [| now apply Hsub1 ].
-      eapply env_locs_monotonic. simpl. rewrite <- !Setminus_Union.
-      reflexivity.
-      eexists (l' |: S1'). split. 
-      now eauto with Ensembles_DB.
-      split. simpl in Hsub1; rewrite <- !Setminus_Union in Hsub1.
-      eapply closed_alloc_Union; simpl; eauto. simpl.
-      rewrite Union_Empty_set_neut_r, Union_Empty_set_neut_l.
-      eapply Singleton_Included...
-      eapply Included_trans. now eapply env_locs_set_Inlcuded'.
-      now eauto with Ensembles_DB.
-    - simpl in Hsub1.
-      rewrite Setminus_Empty_set_neut_r in Hsub1; inv Heq.
-      eexists. split; eauto. reflexivity.
-  Qed.
-    
-  Lemma res_equiv_get_Constr (H1 H2 : heap block)
-        (l1 l2 : loc) (c : cTag) (vs1 : list value) :
-    (Loc l1, H1) ≈ (Loc l2, H2) ->
-    get l1 H1 = Some (Constr c vs1) ->
-    exists vs2,
-      get l2 H2 = Some (Constr c vs2) /\
-      Forall2 (fun v1 v2 => (v1, H1) ≈ (v2, H2)) vs1 vs2.
-  Proof.
-    intros Hres Hget. 
-    rewrite res_equiv_eq in Hres. simpl in Hres. rewrite Hget in Hres.
-    destruct (get l2 H2); try contradiction.
-    destruct b; try contradiction. 
-    destruct Hres as [Heq Hb]. subst. eexists; split; eauto. 
-  Qed.
-
-  Lemma heap_env_equiv_env_get (S : Ensemble var) (H1 H2 : heap block)
-        (rho1 rho2 : env) (x : var) (l : value) :
-    M.get x rho1 = Some l ->
-    S |- (H1, rho1) ⩪ (H2, rho2) ->
-    x \in S ->
-    exists l',
-      M.get x rho2 = Some l' /\
-      (l, H1) ≈ (l', H2).
-  Proof.
-    intros Hget Heq Hin.
-    eapply Heq in Hget; eassumption.
-  Qed.
-  
-  Lemma heap_env_equiv_env_getlist (S : Ensemble var) (H1 H2 : heap block)
-        (rho1 rho2 : env) (xs : list var) (ls : list value) :
-    getlist xs rho1 = Some ls ->
-    S |- (H1, rho1) ⩪ (H2, rho2) ->
-    (FromList xs) \subset S ->
-    exists ls',
-      getlist xs rho2 = Some ls' /\
-      Forall2 (fun l l' => (l, H1) ≈ (l', H2)) ls ls'.
-  Proof with now eauto with Ensembles_DB.
-    revert ls; induction xs; intros ls Hget Heq Hin.
-    - inv Hget.
-      eexists; split; eauto. reflexivity.
-    - simpl in Hget.
-      destruct (M.get a rho1) as [l1 | ] eqn:Hgetl1; try discriminate.
-      destruct (getlist xs rho1) as [ls1 | ] eqn:Hetls1; try discriminate.
-      inv Hget.
-      edestruct heap_env_equiv_env_get as [l2 [Hgetl2 Heq']]; eauto.
-      eapply Hin. rewrite FromList_cons...
-      edestruct IHxs as [ls2 [Hgetls2 Hall2]]; eauto.
-      eapply Included_trans; try eassumption. 
-      rewrite FromList_cons...
-      eexists; split. simpl. rewrite Hgetl2, Hgetls2.
-      reflexivity. constructor; eauto.
-  Qed.
-  
-  Lemma block_equiv_Constr (H1 H2 : heap block) (c : cTag) (vs vs' : list value) :
-    Forall2 (fun l1 l2 => (l1, H1) ≈ (l2, H2)) vs vs' ->
-    block_equiv (H1, Constr c vs) (H2, Constr c vs').
-  Proof.
-    simpl; split; eauto.
-  Qed.
-
-  Lemma block_equiv_Fun (H1 H2 : heap block) (rho1 rho2 : env) :
-    Full_set _ |- (H1, rho1) ⩪ (H2, rho2) ->
-    block_equiv (H1, Env rho1) (H2, Env rho2).
-  Proof.
-    simpl; eauto.
-  Qed.
-
-
-  Lemma heap_env_equiv_getlist_Forall2 S H1 H2 ys vs1 vs2 rho1 rho2 :
-    S |- (H1, rho1) ⩪ (H2, rho2) ->
-    FromList ys \subset S ->
-    getlist ys rho1 = Some vs1 ->
-    getlist ys rho2 = Some vs2 ->
-    Forall2 (fun l1 l2 => (l1, H1) ≈ (l2, H2)) vs1 vs2.
-  Proof.
-    revert vs1 vs2; induction ys; intros vs1 vs2 Heq Hin Hg1 Hg2;
-    destruct vs1; destruct vs2; simpl in *; try discriminate; try now constructor.
-    - destruct (M.get a rho1) eqn:Heqa;
-      destruct (getlist ys rho1) eqn:Heqys; try discriminate.
-    - destruct (M.get a rho2) eqn:Heqa;
-      destruct (getlist ys rho2) eqn:Heqys; try discriminate.
-    - rewrite FromList_cons in Hin.
-      destruct (M.get a rho1) eqn:Heqa;
-        destruct (getlist ys rho1) eqn:Heqys; try discriminate. inv Hg1.
-      eapply Heq in Heqa. destruct Heqa as [l' [Hget Heq']].
-      rewrite Hget in Hg2.
-      destruct (getlist ys rho2) eqn:Heqys'; try discriminate. inv Hg2.
-      constructor; eauto. eapply IHys; eauto.
-      eapply Included_trans; now eauto with Ensembles_DB.
-      eapply Included_trans; now eauto with Ensembles_DB.
-  Qed.
-  
-
-  Lemma reach_env_locs_alloc_not_In S H H' rho x b l :
-    alloc b H = (l, H') ->
-    locs b \subset (reach' H (env_locs rho S)) ->
-    ~ x \in S ->
-    Union _ [set l] (reach' H (env_locs rho S)) \subset
-    reach' H' (env_locs (M.set x (Loc l) rho) (Union _ S [set x])).
-  Proof.
-    intros Hal Hsub Hnin l1 Hin.
-    rewrite <- (env_locs_set_not_In) with (l := Loc l) in Hin; eauto.
-    rewrite env_locs_Union, reach'_Union. inv Hin.
-    - inv H0. right. exists 0. split. 
-      now constructor. simpl. eexists. split; eauto.
-      reflexivity. now rewrite M.gss.
-    - left. eapply reach'_heap_monotonic; eauto.
-      eapply alloc_subheap. eassumption.
-  Qed.
-
-  (* XXX fix *)
-  (* Lemma heap_env_approx_Vfun S H H'  rho rho' rho1 rho2 l l' f f' B : *)
-  (*   M.get f rho = Some (FunPtr l f') -> *)
-  (*   M.get f rho' = Some (FunPtr l' f') -> *)
-  (*   (FunPtr l f', H) ≈ (FunPtr l' f', H') -> *)
-  (*   S |- (H, rho) ⩪ (H', rho') -> *)
-  (*   f \in S -> *)
-  (*   get l H = Some (Vfun rho1 B) -> *)
-  (*   get l' H' = Some (Vfun rho2 B) -> *)
-  (*   heap_env_approx (occurs_free_fundefs B) (H, rho1) (H', rho2). *)
-  (* Proof. *)
-  (*   intros Hget1 Hget2 Heq Hheq Hin Hget1' Hget2' x1 l1 Hin' Hget. *)
-  (*   edestruct Heq with (n := 1) as [[_ Heq1] [_ Heq2]].  *)
-  (*   edestruct Heq1 as [rho2' [Hget' Hlt]]; eauto. *)
-  (*   destruct (Hlt 0 x1) as [[l1' [l2' [Hgetl1 [Hgetl2 _]]]] | [Hn1 Hn2]]; eauto; *)
-  (*   try congruence. *)
-  (*   rewrite Hget in Hgetl1; inv Hgetl1. rewrite Hget2' in Hget'. inv Hget'. *)
-  (*   eexists; split; eauto. *)
-  (*   intros n. *)
-  (*   edestruct Heq with (n := n + 1) as [[_ Heqn1] [_ Heqn2]]. *)
-  (*   split. *)
-  (*   - edestruct Heqn1 as [rho2 [Hget' Hlt']]; eauto. *)
-  (*     rewrite Hget2' in Hget'; inv Hget'. *)
-  (*     destruct (Hlt' n x1) as [[l3' [l4' [Hgetl3 [Hgetl4 Hres]]]] | [Hn1 Hn2]]; eauto; *)
-  (*     try congruence. *)
-  (*     omega. *)
-  (*     rewrite Hgetl3 in Hget; inv Hget. *)
-  (*     rewrite Hgetl4 in Hgetl2; inv Hgetl2. *)
-  (*     rewrite <- res_approx_fuel_eq. eassumption. *)
-  (*   - edestruct Heqn2 as [rho2 [Hget' Hlt']]; eauto. *)
-  (*     rewrite Hget1' in Hget'; inv Hget'. *)
-  (*     destruct (Hlt' n x1) as [[l3' [l4' [Hgetl3 [Hgetl4 Hres]]]] | [Hn1 Hn2]]; eauto; *)
-  (*     try congruence. *)
-  (*     omega. *)
-  (*     rewrite Hgetl3 in Hgetl2; inv Hgetl2. *)
-  (*     rewrite Hgetl4 in Hget; inv Hget. *)
-  (*     rewrite <- res_approx_fuel_eq. eassumption. *)
-  (* Qed. *)
-
-  (* Corollary heap_env_equiv_Vfun S rho rho' rho1 rho2 H H' l l' f f' B : *)
-  (*   M.get f rho = Some (FunPtr l f') -> *)
-  (*   M.get f rho' = Some (FunPtr l' f') -> *)
-  (*   (FunPtr l f', H) ≈ (FunPtr l' f', H') -> *)
-  (*   S |- (H, rho) ⩪ (H', rho') -> *)
-  (*   f \in S -> *)
-  (*   get l H = Some (Vfun rho1 B) -> *)
-  (*   get l' H' = Some (Vfun rho2 B) -> *)
-  (*   (occurs_free_fundefs B) |- (H, rho1) ⩪ (H', rho2). *)
-  (* Proof. *)
-  (*   intros. split. *)
-  (*   now eapply (heap_env_approx_Vfun _ H H' rho rho'); eauto. *)
-  (*   now eapply (heap_env_approx_Vfun _ H' H rho' rho); eauto; symmetry. *)
-  (* Qed. *)
-
-  (** * Lemmas about [live] *)  
-  Lemma live_exists S H :
-    Decidable S ->
-    exists H', live S H H'.
-  Proof.
-  Admitted.
-  
-  Lemma live_deterministic S H1 H2 H2' :
-    live S H1 H2 ->
-    live S H1 H2' ->
-    S |- H2 ≃ H2'.
-  Proof.
-    intros [Hyp1 [Hyp2 Hyp3]] [Hyp1' [Hyp2' Hyp3']].
-    eapply Equivalence.equiv_transitive; eauto.
-    symmetry. eassumption.
-  Qed.
-
-(*  Lemma live_heap_eq (S : Ensemble loc) (H1 H1' H2 : heap block) :
-    reach' H1 S |- H1 ≡ H1' ->
-    live S H1 H2 ->
-    live S H1' H2.
-  Proof.
-    intros Heq [Hs Hl]. split.
-    - intros l b Hget1. rewrite <- Heq.
-      now edestruct Hs as [b' Hget']; eauto. 
-      assert (Hin : l \in dom H2) by (eexists; eauto).
-      eapply Hl in Hin. now inv Hin.
-    - rewrite Hl. split; intros l Hin.
-      + inv Hin. destruct H0 as [v1 Hget1].
-        constructor. rewrite <- reach'_heap_eq; try eassumption.
-        rewrite Heq in Hget1; eauto. eexists; eauto.
-      + inv Hin. destruct H0 as [v1 Hget1].
-        rewrite <- reach'_heap_eq in H; eauto.
-        constructor; try eassumption.
-        rewrite <- Heq in Hget1; eauto. eexists; eauto.
-  Qed.*)
-
-  Lemma live_collect S H1 H2 :
-    live S H1 H2 ->
-    collect S H1 H2.
-  Proof.
-    firstorder.
-  Qed.
-  
-  Lemma live_idempotent (S : Ensemble loc) (H1 H2 : heap block) :
-    live S H1 H2 ->
-    live S H2 H2.
-  Proof.
-    intros Hl.
-    assert (Hc := live_collect _ _ _ Hl).
-    destruct Hl as [Hyp1 [Hyp2 Hyp3]]. split; eauto.
-    split; eauto.
-    reflexivity. 
-  Qed.
-
-  Instance Properlive : Proper (Same_set _ ==> eq ==> eq ==> iff) live.
-  Proof.
-    constructor; subst; intros [Hl1 [Hl2 Hl3]].
-    split; eauto. split; eauto; now rewrite <- H.
-    split; eauto. split; eauto; now rewrite H.
-  Qed.
+    intros Hall. revert n. induction Hall; intros n Hnth1 Hnth2.
+    - now inv Hnth1.
+    - destruct n.
+      + inv Hnth1. inv Hnth2. eassumption.
+      + eapply IHHall; eauto.
+  Qed. 
 
  End HeapDefs.
