theories/L6_PCPS/Heap/heap_equiv.v
@@ -1,0 +1,1485 @@
+(* Heap equivalence definitions for L6. Part of the CertiCoq project.
+ * Author: Zoe Paraskevopoulou, 2016
+ *)
+
+From Coq Require Import NArith.BinNat Relations.Relations MSets.MSets
+         MSets.MSetRBT Lists.List omega.Omega Sets.Ensembles Relations.Relations
+         Classes.Morphisms.
+From ExtLib Require Import Structures.Monad Data.Monads.OptionMonad Core.Type.
+From L6 Require Import cps cps_util eval List_util Ensembles_util functions
+        identifiers Heap.heap tactics Heap.heap_defs.
+Require Import compcert.lib.Coqlib.
+
+Import ListNotations.
+
+Open Scope Ensembles_scope.
+
+Module HeapEquiv (H : Heap).
+  
+  Module Defs := HeapDefs H.
+
+  Import H Defs.
+
+  (** Syntactic approximation of results with fuel *)
+  Fixpoint res_approx_fuel (n : nat) (r1 r2 : res) : Prop :=
+    let '(v1, H1) := r1 in
+    let '(v2, H2) := r2 in
+    match v1, v2 with
+      | Loc l1, Loc l2 => 
+        match get l1 H1 with
+          | Some (Constr c vs1) =>
+            exists vs2, 
+              get l2 H2 = Some (Constr c vs2) /\
+              forall i, (i < n)%nat ->
+                   match n with
+                     | 0%nat => True
+                     | S n' =>
+                       Forall2
+                         (fun l1 l2 => res_approx_fuel (n'-(n'-i)) (l1, H1) (l2, H2)) vs1 vs2
+                   end
+          | Some (Env rho1) =>
+            exists rho2,
+              get l2 H2 = Some (Env rho2) /\
+              (forall x,  (exists v1 v2, M.get x rho1 = Some v1 /\
+                               M.get x rho2 = Some v2 /\
+                               (forall i, (i < n)%nat ->
+                                     match n with
+                                       | 0%nat => True
+                                       | S n' => res_approx_fuel (n'-(n'-i)) (v1, H1) (v2, H2)
+                                     end)) \/
+                     (M.get x rho1 = None /\ M.get x rho2 = None))
+          | None => True
+        end
+      | FunPtr B1 f1, FunPtr B2 f2 => f1 = f2 /\ B1 = B2
+      | _, _ => False
+    end.
+  
+  (** Result equivalence. Two results represent the exact same value *)
+  Definition res_equiv (r1 r2 : res) : Prop :=
+    forall n, res_approx_fuel n r1 r2 /\ res_approx_fuel n r2 r1.
+  
+  Infix "≈" := res_equiv (at level 70, no associativity).
+
+  Definition ans_equiv (a1 a2 : ans) :=
+    match a1, a2 with
+      | Res r1, Res r2 => r1 ≈ r2
+      | OOT, OOT => True
+      | _, _  => False
+    end.
+  
+  (** Approximation lifted to the environments *)
+  Definition heap_env_approx (S : Ensemble var) p1 p2 : Prop :=
+    let '(H1, rho1) := p1 in
+    let '(H2, rho2) := p2 in
+    forall x l, x \in S ->
+           M.get x rho1 = Some l ->
+           exists l', M.get x rho2 = Some l' /\
+                 (l, H1) ≈ (l', H2).
+  
+  (** Equivalence lifted to the environments *)
+  Definition heap_env_equiv S p1 p2 : Prop :=
+    heap_env_approx S p1 p2 /\
+    heap_env_approx S p2 p1.
+  
+  Notation "S |- p1 ⩪ p2" := (heap_env_equiv S p1 p2)
+                               (at level 70, no associativity).
+  
+  Definition block_equiv (p1 p2 : heap block * block) :=
+    let '(H1, b1) := p1 in
+    let '(H2, b2) := p2 in
+    match b1, b2 with
+      | Constr c1 vs1, Constr c2 vs2 =>
+        c1 = c2 /\ Forall2 (fun v1 v2 => (v1, H1) ≈ (v2, H2)) vs1 vs2
+      | Env rho1, Env rho2 => Full_set _ |- (H1, rho1) ⩪ (H2, rho2)
+      | _, _ => False
+    end.
+  
+  Definition heap_approx (S : Ensemble loc) H1 H2 : Prop :=
+    forall b1 l, l \in S -> get l H1 = Some b1 ->
+           exists b2, get l H2 = Some b2 /\ block_equiv (H1, b1) (H2, b2).
+  
+  Definition heap_equiv (S : Ensemble loc) H1 H2 : Prop :=
+    heap_approx S H1 H2 /\ heap_approx S H2 H1. 
+
+  Notation  "S |- H1 ≃ H2" := (heap_equiv S H1 H2)
+                                (at level 70, no associativity).
+  
+  (** Equivalent definition, unfolding the recursion *)
+  Definition res_approx_fuel' (n : nat) (r1 r2 : res) : Prop :=
+    let '(v1, H1) := r1 in
+    let '(v2, H2) := r2 in
+    match v1, v2 with
+      | Loc l1, Loc l2 => 
+        match get l1 H1 with
+          | Some (Constr c vs1) =>
+            exists vs2, 
+              get l2 H2 = Some (Constr c vs2) /\
+              forall i, (i < n)%nat ->
+                   Forall2 (fun l1 l2 => res_approx_fuel i (l1, H1) (l2, H2)) vs1 vs2
+          | Some (Env rho1) =>
+            exists rho2,
+              get l2 H2 = Some (Env rho2) /\
+               (forall x, (exists v1 v2, M.get x rho1 = Some v1 /\
+                               M.get x rho2 = Some v2 /\
+                               (forall i, (i < n)%nat ->
+                                     res_approx_fuel i (v1, H1) (v2, H2))) \/
+                     (M.get x rho1 = None /\ M.get x rho2 = None))
+          | None => True
+        end
+      | FunPtr B1 f1, FunPtr B2 f2 => f1 = f2 /\ B1 = B2
+      | _, _ => False
+    end.
+  
+  (** Equivalence of the two definitions *)
+  Lemma res_approx_fuel_eq n r1 r2 :
+    res_approx_fuel n r1 r2 <-> res_approx_fuel' n r1 r2.
+  Proof.
+    destruct n; destruct r1 as [[l1 | B1 f1] H1]; destruct r2 as [[l2 | B2 f2] H2]; simpl.
+    - destruct (get l1 H1) as [[c1 vs1 | rho1]|]; [| | now firstorder ].
+      + split.
+        * intros [vs [H _ ]]. eexists. split; eauto.
+          intros; omega.
+        * intros [vs [H _ ]]. eexists. split; eauto.
+      + split.
+        * intros [vs [H Hb ]]. eexists. split; eauto.
+          intros x. destruct (Hb x) as [Hb1 | Hb1]; eauto. 
+          destruct Hb1 as [v1 [v2 [Hget1 [Hget2 Ht]]]].
+          left. repeat eexists; eauto. intros; omega.
+        * intros [vs [H Hb ]]. eexists. split; eauto.
+          intros x. destruct (Hb x) as [Hb1 | Hb1]; eauto. 
+          destruct Hb1 as [v1 [v2 [Hget1 [Hget2 Ht]]]].
+          left. repeat eexists; eauto.
+    - split; eauto.
+    - split; eauto.   
+    - now firstorder.
+    - destruct (get l1 H1) as [[c1 vs1 | rho1 ]|]; [| | now firstorder ].
+      + split.
+        * intros [vs [H Hi]]. eexists. split; eauto.
+          intros i Hlt.
+          assert (Heq : (i =  n - (n - i))%nat) by omega. rewrite Heq.
+          eauto.
+        * intros [vs [H Hin]]. eexists. split; eauto.
+          intros i Hlt.
+          assert (Heq : (i =  n - (n - i))%nat) by omega. rewrite <- Heq.
+          eauto.
+      + split.
+        * intros [vs [H Hb ]]. eexists. split; eauto.
+          intros x. destruct (Hb x) as [Hb1 | Hb1]; eauto. 
+          destruct Hb1 as [v1 [v2 [Hget1 [Hget2 Ht]]]].
+          left. repeat eexists; eauto.
+          intros i Hlt.
+          assert (Heq : (i =  n - (n - i))%nat) by omega. rewrite Heq.
+          eauto.
+        * intros [vs [H Hb ]]. eexists. split; eauto.
+          intros x. destruct (Hb x) as [Hb1 | Hb1]; eauto. 
+          destruct Hb1 as [v1 [v2 [Hget1 [Hget2 Ht]]]].
+          left. repeat eexists; eauto.
+          intros i Hlt.
+          assert (Heq : (i =  n - (n - i))%nat) by omega. rewrite <- Heq.
+          eauto.
+    - split; eauto.
+    - split; eauto.   
+    - now firstorder.
+  Qed.
+
+  Opaque res_approx_fuel.
+  
+ (** Equivalent definition for [res_equiv] *)
+  Definition res_equiv' (r1 r2 : res) : Prop :=
+    let '(v1, H1) := r1 in
+    let '(v2, H2) := r2 in
+    match v1, v2 with
+      | Loc l1, Loc l2 =>
+        match get l1 H1, get l2 H2 with
+          | Some b1, Some b2 => block_equiv (H1, b1) (H2, b2)
+          | None, None => True
+          | _, _ => False
+        end
+      | FunPtr B1 f1, FunPtr B2 f2 =>
+        B1 = B2 /\ f1 = f2
+      | _, _ => False
+    end.
+
+  
+  Lemma res_equiv_eq r1 r2 :
+    res_equiv r1 r2 <-> res_equiv' r1 r2.
+  Proof.
+    destruct r1 as [[l1 | B1 f1] H1]; destruct r2 as [[l2 | B2 f2] H2]; simpl.
+    unfold res_equiv. split. 
+    - intros H. assert (H0 := H 0%nat).
+      destruct H0 as [Hal Har]. rewrite !res_approx_fuel_eq in Hal, Har.
+      simpl in *. destruct (get l1 H1) as [ v |] eqn:Hget1.
+      + destruct v as [c1 vs1 | rho1 B1 off1 ].
+        * destruct Hal as [vs2 [Hget2 Hi]].
+          rewrite Hget2 in Har.
+          destruct Har as [vs1' [Hget1' Hi']]. inv Hget1'. 
+          rewrite Hget2. split; eauto.
+          eapply Forall2_forall. constructor. exact 0%nat.
+          intros n. specialize (H (S n)). rewrite !res_approx_fuel_eq in H. 
+          edestruct H as [Hal' Har']. simpl in Hal', Har'.
+          rewrite Hget1 in Hal'. rewrite Hget2 in Har'. 
+          destruct Hal' as [vs2' [Hget2' Hi2]]. subst_exp.
+          destruct Har' as [vs1 [Hget1' Hi1]]. subst_exp.
+          eapply Forall2_conj.
+          eapply Hi2. omega.
+          eapply Forall2_flip. eapply Hi1. omega.
+        * destruct Hal as [rho2 [Hget2 Hi1]].
+          rewrite Hget2 in Har.
+          destruct Har as [rho1' [Hget1' Hi2]]. inv Hget1'. 
+          rewrite Hget2. split; eauto; intros x l _ Hget.
+          { destruct (Hi1 x) as [[v1 [v2 [Hgetv1 [Hgetv2 Hi]]]] | [Hn1 Hn2]]; try congruence.
+            subst_exp. eexists; split; eauto.
+            intros n.
+            specialize (H (S n)). rewrite !res_approx_fuel_eq in H. 
+            edestruct H as [Hal' Har']. simpl in Hal', Har'.
+            rewrite Hget1 in Hal'. rewrite Hget2 in Har'. 
+            destruct Hal' as [rho2' [Hget2' Hin2]]. subst_exp.
+            destruct Har' as [rho1 [Hget1' Hin1]]. subst_exp.
+            destruct (Hin1 x) as [[v1' [v2' [Hgetv1' [Hgetv2' Hi1']]]] | [Hn1 Hn2]]; try congruence.
+            repeat subst_exp.
+            destruct (Hin2 x) as [[v1'' [v2'' [Hgetv1' [Hgetv2' Hi2']]]] | [Hn1 Hn2]]; try congruence.
+            repeat subst_exp. split; eauto. }
+          { destruct (Hi1 x) as [[v1 [v2 [Hgetv1 [Hgetv2 Hi]]]] | [Hn1 Hn2]]; try congruence.
+            subst_exp. eexists; split; eauto.
+            intros n.
+            specialize (H (S n)). rewrite !res_approx_fuel_eq in H. 
+            edestruct H as [Hal' Har']. simpl in Hal', Har'.
+            rewrite Hget1 in Hal'. rewrite Hget2 in Har'. 
+            destruct Hal' as [rho2' [Hget2' Hin2]]. subst_exp.
+            destruct Har' as [rho1 [Hget1' Hin1]]. subst_exp.
+            destruct (Hin1 x) as [[v1' [v2' [Hgetv1' [Hgetv2' Hi1']]]] | [Hn1 Hn2]]; try congruence.
+            repeat subst_exp.
+            destruct (Hin2 x) as [[v1'' [v2'' [Hgetv1' [Hgetv2' Hi2']]]] | [Hn1 Hn2]]; try congruence.          
+            repeat subst_exp. split; eauto. }
+      + destruct (get l2 H2); eauto.
+        destruct b.
+        destruct Har as [vs2 [Heq _]]; discriminate.
+        destruct Har as [vs2 [Heq _]]; discriminate.
+    - destruct (get l1 H1) eqn:Hget1.
+      + destruct b as [ c vs1 | rho1 B1 off1 ].
+        * destruct (get l2 H2) eqn:Hget2; try contradiction.
+          destruct b as [c' vs2 |]; try contradiction.
+          intros [Heq Hall] n. subst. rewrite !res_approx_fuel_eq.
+          simpl. rewrite Hget1, Hget2. split.
+          
+          eexists. split. reflexivity.
+          intros. eapply Forall2_monotonic; [| eassumption ].
+          now intros v1 v2 [Hl Hr]; eauto. 
+
+          eexists. split. reflexivity.
+          intros. eapply Forall2_flip. eapply Forall2_monotonic; [| eassumption ].
+          now intros v1 v2 [Hl Hr]; eauto. 
+        * destruct (get l2 H2) eqn:Hget2; try contradiction.
+          destruct b as [ | rho2]; try contradiction.
+          intros [Hl Hr] n. rewrite !res_approx_fuel_eq.
+          simpl. rewrite Hget1, Hget2. split.
+          
+          eexists. split. reflexivity.
+          intros x.
+          destruct (M.get x rho1) as [v1|] eqn:Hgetv1.
+          edestruct Hl as [v2 [Hgetv2 Hi]]; try eassumption.
+          now constructor.
+          left; repeat eexists; eauto. intros. now eapply Hi.
+          destruct (M.get x rho2) as [v2|] eqn:Hgetv2; eauto.
+          edestruct Hr as [v1 [Hgetv1' Hi']]; try eassumption.
+          now constructor. congruence.
+          
+          eexists. split. reflexivity.
+          intros x.
+          destruct (M.get x rho1) as [v1|] eqn:Hgetv1.
+          edestruct Hl as [v2 [Hgetv2 Hi]]; try eassumption.
+          now constructor.
+          left; repeat eexists; eauto. intros. now eapply Hi.
+          destruct (M.get x rho2) as [v2|] eqn:Hgetv2; eauto.
+          edestruct Hr as [v1 [Hgetv1' Hi']]; try eassumption.
+          now constructor. congruence.
+      + destruct (get l2 H2) eqn:Hget2; try contradiction.
+        intros. rewrite !res_approx_fuel_eq. simpl.
+        rewrite Hget1, Hget2; eauto.
+    - split; try contradiction.
+      intros Heq. destruct (Heq 0%nat) as [Hl Hr].
+      rewrite res_approx_fuel_eq in *. contradiction.
+    - split; try contradiction.
+      intros Heq. destruct (Heq 0%nat) as [Hl Hr].
+      rewrite res_approx_fuel_eq in *. contradiction.
+    - split.
+      + intros Heq. destruct (Heq 0%nat) as [Hl Hr].
+        rewrite res_approx_fuel_eq in *. inv Hl. split; eauto.
+      + intros [Hl1 Hr2]; subst.
+        split; eauto; rewrite res_approx_fuel_eq; simpl; split; eauto.  
+  Qed.
+
+
+  (** Using S as the set of roots, garbage collect H1 *) 
+  Definition collect (S : Ensemble loc) (H1 H2 : heap block) : Prop :=
+    size_heap H2 <= size_heap H1 /\
+    S |- H1 ≃ H2. (* locations outside S might be renamed! *)
+  
+  (** [live S H1 H2] iff H2 is the live portion of H1, using S as roots *)
+  Definition live (S : Ensemble loc) (H1 H2 : heap block) : Prop :=
+    size_heap H2 <= size_heap H1 /\ (* maybe could be derived *)
+    heap_equiv S H1 H2 /\ (* locations outside S might be renamed! *)
+    dom H2 \subset reach' H2 S. (* everything in the domain is reachable *)
+
+  (** The size of the reachable portion of the heap *)
+  Definition size_reach (H : heap block) (S : Ensemble loc) (n : nat) : Prop :=
+    forall H', live S H H' -> size_heap H' = n. 
+
+  (** * Lemmas about [collect] *)
+  
+  (** The reachable part of the heap before and after collection are the same *)
+  Lemma collect_heap_eq S H1 H2 :
+    collect S H1 H2 ->
+    S |- H1 ≃ H2.
+  Proof.
+    firstorder.
+  Qed.
+  
+  Lemma collect_size S H1 H2 :
+    collect S H1 H2 ->
+    size_heap H2 <= size_heap H1.
+  Proof.
+    now firstorder.
+  Qed.
+  
+
+  (** * Lemmas about [reach_size] *)
+
+(*
+  Lemma size_reach_heap_eq (S : Ensemble loc) (H1 H1' : heap block) (m : nat) :
+    reach' H1 S |- H1 ≡ H1' ->
+    size_reach H1 S m ->
+    size_reach H1' S m.
+  Proof.
+    intros Heq Hs H2 Hl. eapply Hs.
+    eapply live_heap_eq; eauto. rewrite <- reach'_heap_eq; eauto.
+    now symmetry.
+  Qed.
+ *)
+
+  (** * Lemmas about [res_approx] and [res_equiv] *)
+
+  (** Preorder and equivalence properties of [res_approx] and [res_equiv] *)
+
+  Lemma heap_equiv_res_approx (S : Ensemble loc) (H1 H2 : heap block)
+        (v : value) (n : nat) :
+    S |- H1 ≃ H2  ->
+    (val_loc v) \subset S -> 
+    res_approx_fuel n (v, H1) (v, H2).
+  Proof.
+    intros [Heq1 Heq2] Hin.
+    destruct v as [l | B f]; rewrite res_approx_fuel_eq; [| now split; eauto ].
+    simpl; destruct (get l H1) eqn:Hget; eauto.
+    eapply Heq1 in Hget; eauto.
+    destruct Hget as [b2 [Hget2 Heq]].
+    destruct b; destruct b2; try contradiction.
+    - destruct Heq as [Heq Hin2]; subst. eexists; split; eauto. 
+      intros. 
+      eapply Forall2_monotonic; eauto. simpl.
+      intros ? ? [Ha1 Ha2]; eauto.
+    - eexists; split; eauto. 
+      intros x. destruct Heq as [Hal Har].
+      destruct (M.get x e) eqn:Hgetx1; destruct (M.get x e0) eqn:Hgetx2;
+      simpl in *; eauto.
+      + left. repeat eexists; eauto.
+        edestruct Hal as [l' [Hgetx2' Ha]]; eauto.
+        now constructor. subst_exp. intros i Hleq; destruct (Ha i); eassumption.
+      + edestruct Hal as [l' [Hgetx2' Ha]]; eauto.
+        now constructor. congruence.
+      + edestruct Har as [l' [Hgetx2' Ha]]; eauto.
+        now constructor. congruence.
+    - eapply Hin. reflexivity. 
+  Qed.
+
+  Lemma Preorder_res_approx_fuel i : preorder res (res_approx_fuel i).
+  Proof.
+    constructor.
+    - induction i as [i IHi] using lt_wf_rec.
+      intros [v H1]. rewrite res_approx_fuel_eq. destruct v.
+      simpl. destruct (get l H1) eqn:Hgetl; eauto. 
+      destruct b as [c vs | rho B f]. 
+      + eexists; split; eauto.
+        intros i' Hlt.
+        eapply Forall2_refl; intros l'. eapply IHi. eassumption.
+      + eexists; split; eauto. 
+        intros x.
+        destruct (M.get x rho) eqn:heq; eauto.
+        * left. do 2 eexists; repeat split; eauto.
+          intros. eapply IHi; eauto.
+      + split; eauto.
+    - induction i as [i IHi]  using lt_wf_rec1.
+      intros [v1 H1] [v2 H2] [v3 H3] Hap1 Hap2. rewrite res_approx_fuel_eq in *.
+      simpl in *.
+      destruct v1 as [l1 | B1 f1]; destruct v2 as [l2 | B2 f2]; destruct v3 as [l3 | B3 f3];
+      try contradiction.
+      { destruct (get l1 H1) eqn:Hget1; eauto.
+        destruct b as [c vs1 | rho1 B f].
+        + edestruct Hap1 as [vs2 [Hget2 Hall2]]. rewrite Hget2 in Hap2.
+          destruct Hap2 as [vs3 [Hget3 Hall3]].
+          eexists; split; eauto.
+          intros i' Hlt.
+          eapply Forall2_trans_strong; eauto. intros v1 v2 v3 Hv1 Hv2.
+          eapply IHi. eassumption. simpl in Hv1. eassumption.
+          simpl in Hv2. eassumption.
+        + edestruct Hap1 as [rho2 [Hget2 Hall2]]. rewrite Hget2 in Hap2.
+          destruct Hap2 as [rho33 [Hget3 Hall3]].
+          eexists; split; eauto.
+          intros x.
+          edestruct Hall2 as [[l1' [l2' [Hgetl1 [Hgetl2 Hi]]]] | [Hn1 Hn2]]; eauto.
+          * edestruct Hall3 as [[l2'' [l3' [Hgetl2' [Hgetl3 Hi']]]] | [Hn1 Hn2]]; eauto.
+            repeat subst_exp.
+            left; repeat eexists; eauto. subst_exp.
+            intros. eapply IHi; eauto.
+            congruence.
+          * edestruct Hall3 as [[l2'' [l3' [Hgetl2' [Hgetl3 Hi']]]] | [Hn2' Hn3]]; eauto.
+            congruence. }
+      { inv Hap1; inv Hap2. split; eauto. }
+  Qed.
+
+  Instance Equivalence_res_equiv : Equivalence res_equiv.
+  Proof.
+    constructor. 
+    - intros res; split; eapply Preorder_res_approx_fuel.
+    - intros res res' H n. destruct (H n) as [H1 H2]. split; eauto.
+    - intros res1 res2 res3 H1 H2. intros n.
+      destruct (H1 n) as [Ht1 Ht2]; destruct (H2 n) as [Ht3 Ht4];
+      split.
+      now eapply Preorder_res_approx_fuel; eauto.
+      now eapply Preorder_res_approx_fuel; eauto.
+  Qed.
+  
+  Instance Equivalence_heap_env_equiv S : Equivalence (heap_env_equiv S).
+  Proof.
+    constructor.
+    - intros [H rho]; split; intros l Hget; eexists; split; eauto; reflexivity.
+    - intros [H rho] [H' rho'] H1; split; intros v l Hin Hget;
+      eapply H1; eauto.
+    - edestruct Equivalence_res_equiv; eauto.
+      intros [H rho] [H' rho'] [H'' rho''] H1 H2; split; intros v l Hin Hget.
+      edestruct H1 as [H1' _]; eauto. edestruct H1' as [v1 [Hget1 Hres1]]; eauto.
+      edestruct H2 as [H2' _]; eauto. edestruct H2' as [v2 [Hget2 Hres2]]; eauto.
+      edestruct H2 as [_ H2']; eauto. edestruct H2' as [v2 [Hget2 Hres2]]; eauto.
+      edestruct H1 as [_ H1']; eauto. edestruct H1' as [v1 [Hget1 Hres1]]; eauto.
+  Qed.
+
+  (** * Lemmas about [block_equiv] **)
+  
+  Instance Reflexive_block_equiv : Reflexive block_equiv.
+  Proof.
+    intros [H b]. destruct b; simpl; eauto; try reflexivity.
+    split; eauto. eapply Forall2_refl; now eauto with typeclass_instances.
+  Qed.
+  
+  Instance Transitive_block_equiv : Transitive block_equiv.
+  Proof.
+    intros [H1 b1] [H2 b2] [H3 b3] Hb1 Hb2.
+    destruct b1; destruct b2; try contradiction;
+    destruct b3; try contradiction.
+    - destruct Hb1 as [Heq1 Hb1].
+      destruct Hb2 as [Heq2 Hb2].
+      subst. split; eauto. 
+      eapply Forall2_trans_strong; try eassumption.
+      simpl; intros. eapply Equivalence_Transitive; eauto. 
+    - simpl in *.
+      eapply Equivalence_Transitive; eauto.
+  Qed.
+  
+  Instance Symmetric_block_equiv : Symmetric block_equiv.
+  Proof.
+    intros [H1 b1] [H2 b2] Hb.
+    destruct b1; destruct b2; try contradiction.
+    - destruct Hb as [Heq1 Hb1].
+      subst. split; eauto. 
+      eapply Forall2_symm_strong; try eassumption.
+      simpl; intros. symmetry. eauto.
+    - simpl in *. symmetry; eauto.
+  Qed.
+
+  Instance Equivalence_heap_equiv S : Equivalence (heap_equiv S). 
+  Proof.
+    constructor.
+    - intros H.
+      split; intros x l Hin Hget;
+      eexists; split; eauto; reflexivity.
+    - intros H1 H2 [Hs1 Hs2].
+      split; intros x l Hin Hget. 
+      edestruct (Hs2 x l Hin Hget) as [b1 [Hget1 Heq1]]. 
+      eexists; split; eauto; symmetry; eauto.
+      edestruct (Hs1 x l Hin Hget) as [b1 [Hget1 Heq1]]. 
+      eexists; split; eauto; symmetry; eauto.
+    - intros H1 H2 H3 [Hs1 Hs2] [Hs2' Hs3].
+      split; intros x l Hin Hget. 
+      edestruct (Hs1 x l Hin Hget) as [b1 [Hget1 Heq1]]. 
+      edestruct (Hs2' _ _ Hin Hget1) as [b2 [Hget2 Heq2]].
+      eexists; split; eauto. now eapply Transitive_block_equiv; eauto.
+      edestruct (Hs3 x l Hin Hget) as [b1 [Hget1 Heq1]]. 
+      edestruct (Hs2 _ _ Hin Hget1) as [b2 [Hget2 Heq2]].
+      eexists; split; eauto. eapply Transitive_block_equiv; eauto.
+  Qed.
+
+
+  Lemma heap_env_approx_heap_equiv (S : Ensemble var) (H1 H2 : heap block) (rho : env) : 
+    (env_locs rho S) |- H1 ≃ H2 -> 
+    heap_env_approx S (H2, rho) (H1, rho).
+  Proof.
+    intros [Heq1 Heq2] x v Hin Hget.
+    eexists; split; eauto.  
+    rewrite res_equiv_eq. simpl.
+    destruct v as [l | B f]; [| now split; eauto ].
+    destruct (get l H1) eqn:Heq.
+    - eapply Heq1 in Heq.
+      destruct Heq as [b2 [Hb2 Heqb]]. rewrite Hb2.
+      simpl in Heqb. destruct b; destruct b2; try contradiction.
+      destruct Heqb as [Heqc Hall]; subst; split; eauto.
+      eapply Forall2_symm_strong; eauto.
+      simpl; intros.
+      now eapply Equivalence.equiv_symmetric; eauto.
+      now symmetry; eauto. eapply get_In_env_locs; eauto.
+      reflexivity.
+    - destruct (get l H2) eqn:HgetH2; eauto.
+      eapply Heq2 in HgetH2.
+      destruct HgetH2 as [b2 [Hgetb2 _]].
+      congruence.
+      eexists; split; eauto. rewrite Hget; eauto. reflexivity.
+  Qed.   
+  
+  Corollary heap_env_equiv_heap_equiv (S : Ensemble var) (H1 H2 : heap block)
+            (rho : env) :
+    (env_locs rho S) |- H1 ≃ H2 -> 
+    S |- (H1, rho) ⩪ (H2, rho).
+  Proof.
+    intros. split; eapply heap_env_approx_heap_equiv; simpl; try eassumption.
+    symmetry. eassumption.
+  Qed.
+
+  Lemma heap_equiv_res_equiv (S : Ensemble loc) (H1 H2 : heap block)
+        (v : value) :
+    S |- H1 ≃ H2  ->
+    (val_loc v) \subset S -> 
+    (v, H1) ≈ (v, H2).
+  Proof.
+    intros Heq Hin m.
+    split. eapply heap_equiv_res_approx; eauto. 
+    eapply heap_equiv_res_approx; eauto. symmetry.
+    eassumption. 
+  Qed.
+  
+  (** Proper instances *)
+
+  Instance Proper_heap_env_approx : Proper (Same_set _ ==> eq ==> eq ==> iff) heap_env_approx.
+  Proof.
+    intros s1 s2 hseq p1 p2 Heq p1' p2' Heq'; subst; split; intros H1;
+    destruct p2; destruct p2'; firstorder.
+  Qed.
+
+  Instance Proper_heap_env_equiv : Proper (Same_set _ ==> eq ==> eq ==> iff) heap_env_equiv.
+  Proof.
+    intros s1 s2 hseq p1 p2 Heq p1' p2' Heq'; subst.
+    split; intros [h1 h2]; split; (try now rewrite hseq; eauto);
+    rewrite <- hseq; eauto.
+  Qed.
+
+  Instance Proper_heap_equiv : Proper (Same_set _ ==> eq ==> eq ==> iff) heap_equiv.
+  Proof.
+    intros s1 s2 hseq p1 p2 Heq p1' p2' Heq'; subst.
+    split; intros [h1 h2].
+    split; intros b l HIn; eauto; [eapply h1 | eapply h2]; eapply hseq; eassumption.
+    split; intros b l HIn; eauto; [eapply h1 | eapply h2]; eapply hseq; eassumption.
+  Qed.
+  
+  (** Monotonicity properties *)
+
+  Lemma heap_env_equiv_antimon S1 S2 H1 H2 rho1 rho2 :
+    S1 |- (H1, rho1) ⩪ (H2, rho2) ->
+    S2 \subset S1 ->
+    S2 |- (H1, rho1) ⩪ (H2, rho2).
+  Proof.
+    firstorder.
+  Qed.
+  
+  (** Weakening lemmas *)
+
+  (* TODO move *)
+  Lemma In_Union_list {A} (l : list (Ensemble A)) s:
+    List.In s l ->
+    s \subset Union_list l.
+  Proof.
+    intros Hin. induction l. 
+    - now inv Hin.
+    - inv Hin. now eapply Included_Union_l.
+      simpl. eapply Included_Union_preserv_r.
+      eapply IHl; eauto.
+  Qed.
+
+      
+  Lemma res_approx_weakening (S1 S2 : Ensemble loc) (H1 H2 H1' H2' : heap block)
+        (v1 v2 : value) (i : nat) :
+    closed S1 H1 -> closed S2 H2 ->
+    res_approx_fuel' i (v1, H1) (v2, H2) ->
+    H1 ⊑ H1' -> 
+    H2 ⊑ H2' ->
+    val_loc v1 \subset S1 -> val_loc v2 \subset S2 -> 
+    res_approx_fuel' i (v1, H1') (v2, H2').
+  Proof.
+    intros Hwf1 Hwf2 Heq Hsub1 Hsub2.
+    revert v1 v2 Heq; induction i using lt_wf_rec1;
+    intros v1 v2 Heq Hdom1 Hdom2.
+    destruct v1 as [ l1 | B1 f1]; destruct v2 as [ l2 | V2 f2]; try contradiction. 
+    { edestruct Hwf1 as [b1 [Hget1 Hsub1']].
+      eapply Hdom1; reflexivity. 
+      edestruct Hwf2 as [b2 [Hget2 Hsub2']].
+      eapply Hdom2; reflexivity. 
+      specialize (Hsub1 _ _ Hget1).
+      specialize (Hsub2 _ _ Hget2).
+      simpl in Hget1, Hget2, Hsub1, Heq. 
+      simpl.
+      rewrite Hsub1. rewrite Hget1 in Heq. destruct b1.
+      - edestruct Heq as [vs2 [Hgetl2 Hall]]; eauto.
+        subst_exp.
+      eexists; split; [ now eauto |].
+      intros i' Hlt.
+      eapply Forall2_monotonic_strong
+      with (R :=
+              fun l3 l4 =>
+                val_loc l3 \subset S1 ->
+                val_loc l4 \subset S2 -> res_approx_fuel i' (l3, H1) (l4, H2)).
+      * intros v1' v2' Hin1 Hin2 Hyp. 
+        rewrite res_approx_fuel_eq. eapply H; eauto.
+        rewrite <- res_approx_fuel_eq. eapply Hyp; eauto.
+        simpl in Hsub1'. eapply Included_trans; [| eassumption].
+        eapply In_Union_list. now eapply in_map; eauto.
+        simpl in Hsub2'. eapply Included_trans; [| eassumption].
+        eapply In_Union_list. now eapply in_map; eauto.
+        simpl in Hsub1'. eapply Included_trans; [| eassumption].
+        eapply In_Union_list. now eapply in_map; eauto.
+        simpl in Hsub2'. eapply Included_trans; [| eassumption].
+        eapply In_Union_list. now eapply in_map; eauto.
+      * eapply Forall2_monotonic; [| eauto ].
+        intros. eassumption.
+    - edestruct Heq as [rho2 [Hgetl2 Hall]]; eauto.
+      subst_exp.
+      eexists; split; [ now eauto |].
+      intros x.
+      edestruct Hall as [[v1 [v2 [Hs1 [Hs2 Hi]]]] | Hnone]; eauto.
+      left. repeat eexists; eauto. intros i' Hlt.
+      rewrite res_approx_fuel_eq. eapply H; eauto.
+      rewrite <- res_approx_fuel_eq. eapply Hi. eassumption.
+      simpl in Hsub1'. eapply Included_trans; [| eassumption].
+      eapply get_In_env_locs; eauto. now constructor.
+      simpl in Hsub2'. eapply Included_trans; [| eassumption].
+      eapply get_In_env_locs; eauto. now constructor. }
+    { simpl in *; eassumption. }
+  Qed.
+  
+  Corollary res_equiv_weakening (S1 S2 : Ensemble loc) (H1 H2 H1' H2' : heap block)
+            (v1 v2 : value) :
+    closed S1 H1 -> closed S2 H2 ->
+    (v1, H1) ≈ (v2, H2) ->
+    H1 ⊑ H1' ->
+    H2 ⊑ H2' ->
+    val_loc v1 \subset S1 -> val_loc v2 \subset S2 -> 
+    (v1, H1') ≈ (v2, H2').
+  Proof.
+    intros Hwf1 Hwf2 Heq Hsub1 Hsub2 Hin1 Hin2 n. destruct (Heq n) as [Heq1 He2].
+    split; rewrite res_approx_fuel_eq.
+    eapply (res_approx_weakening S1 S2 H1 H2 H1' H2'); eauto.
+    now rewrite <- res_approx_fuel_eq.
+    eapply (res_approx_weakening S2 S1 H2 H1 H2' H1'); eauto.
+    now rewrite <- res_approx_fuel_eq. 
+  Qed.
+
+
+  Lemma heap_env_approx_weakening S H1 H2 H1' H2' rho1 rho2 :
+    well_formed (reach' H1 (env_locs rho1 S)) H1 ->
+    well_formed (reach' H2 (env_locs rho2 S)) H2 ->
+    env_locs rho1 S \subset dom H1 ->
+    env_locs rho2 S \subset dom H2 ->
+    S |- (H1, rho1) ⩪ (H2, rho2) ->
+    H1 ⊑ H1' ->
+    H2 ⊑ H2' ->
+    heap_env_approx S (H1', rho1) (H2', rho2).
+  Proof.
+    intros Hwf1 Hwf2 He1 He2  [Heq1 Heq2] Hal1 Hal2 y l Hin Hget; simpl.
+    edestruct Heq1 as [x' [Hget' Heq']]; eauto.
+    eexists; split; eauto.
+    eapply (res_equiv_weakening _ _ H1 H2).
+    eapply reach'_closed. now apply Hwf1. eassumption.
+    eapply reach'_closed. now apply Hwf2. eassumption.
+    eassumption. eassumption. eassumption.
+    eapply Included_trans; [| eapply reach'_extensive ].
+    now eapply get_In_env_locs; eauto.
+    eapply Included_trans; [| eapply reach'_extensive ].
+    now eapply get_In_env_locs; eauto.
+  Qed.
+  
+  Corollary heap_env_equiv_weaking_cor S H1 H2 H1' H2' rho1 rho2 :
+    well_formed (reach' H1 (env_locs rho1 S)) H1 ->
+    well_formed (reach' H2 (env_locs rho2 S)) H2 ->
+    env_locs rho1 S \subset dom H1 ->
+    env_locs rho2 S \subset dom H2 ->
+    S |- (H1, rho1) ⩪ (H2, rho2) ->
+    H1 ⊑ H1' ->
+    H2 ⊑ H2' ->
+    S |- (H1', rho1) ⩪ (H2', rho2).
+  Proof.
+    intros. split.
+    now eapply (heap_env_approx_weakening _ H1 H2); eauto.
+    now eapply (heap_env_approx_weakening _ H2 H1); eauto; symmetry.
+  Qed.
+
+  Lemma heap_env_approx_weakening' S S1 S2 H1 H2 H1' H2' rho1 rho2 :
+     closed S1 H1 -> closed S2 H2 ->
+     env_locs rho1 S \subset S1 ->
+     env_locs rho2 S \subset S2 ->
+     S |- (H1, rho1) ⩪ (H2, rho2) ->
+     H1 ⊑ H1' ->
+     H2 ⊑ H2' ->
+     heap_env_approx S (H1', rho1) (H2', rho2).
+   Proof.
+     intros Hwf1 Hwf2 He1 He2  [Heq1 Heq2] Hal1 Hal2 y l Hin Hget; simpl.
+     edestruct Heq1 as [x' [Hget' Heq']]; eauto.
+     eexists; split; eauto.
+     eapply (res_equiv_weakening _ _ H1 H2); eauto.
+     eapply Included_trans; [| eassumption ].
+     now eapply get_In_env_locs; eauto.
+     eapply Included_trans; [| eassumption ].
+     now eapply get_In_env_locs; eauto.
+   Qed.
+   
+   Corollary heap_env_equiv_weaking' S S1 S2 H1 H2 H1' H2' rho1 rho2 :
+     closed S1 H1 -> closed S2 H2 ->
+     env_locs rho1 S \subset S1 ->
+     env_locs rho2 S \subset S2 ->
+     S |- (H1, rho1) ⩪ (H2, rho2) ->
+     H1 ⊑ H1' ->
+     H2 ⊑ H2' ->
+     S |- (H1', rho1) ⩪ (H2', rho2).
+   Proof.
+     intros. split.
+     now eapply (heap_env_approx_weakening' _ _ _ H1 H2); eauto.
+     now eapply (heap_env_approx_weakening' _ _ _ H2 H1); eauto; symmetry.
+   Qed.
+
+     Lemma res_approx_weakening_alt (S1 S2 : Ensemble loc) (H1 H2 H1' H2' : heap block)
+        (v1 v2 : value) (i : nat) :
+    closed S1 H1 -> closed S2 H2 ->
+    res_approx_fuel' i (v1, H1) (v2, H2) ->
+    H1 ⊑ H1' -> 
+    H2 ⊑ H2' ->
+    (val_loc v1) \subset dom H1 ->
+    (val_loc v2) \subset dom H2 ->
+    post H1 (val_loc v1) \subset S1 ->
+    post H2 (val_loc v2) \subset S2 ->
+    res_approx_fuel' i (v1, H1') (v2, H2').
+  Proof.
+    intros Hwf1 Hwf2 Heq Hsub1 Hsub2.
+    revert v1 v2 Heq; induction i using lt_wf_rec1;
+    intros v1 v2 Heq Hdom1 Hdom2 Hpost1 Hpost2.
+    destruct v1 as [ l1 | B1 f1]; destruct v2 as [ l2 | V2 f2]; try contradiction. 
+    { edestruct Hdom1 as [b1 Hget1]; eauto. reflexivity.
+      edestruct Hdom2 as [b2 Hget2]; eauto. reflexivity.
+      specialize (Hsub1 _ _ Hget1).
+      specialize (Hsub2 _ _ Hget2).
+      simpl in Hget1, Hget2, Hsub1, Heq. 
+      simpl.
+      rewrite Hsub1. rewrite Hget1 in Heq. destruct b1.
+      - edestruct Heq as [vs2 [Hgetl2 Hall]]; eauto.
+        subst_exp.
+        eexists; split; [ now eauto |].
+        intros i' Hlt.
+        eapply Forall2_monotonic_strong
+        with (R :=
+                fun l3 l4 =>
+                  val_loc l3 \subset dom H1 ->
+                  val_loc l4 \subset dom H2 -> res_approx_fuel i' (l3, H1) (l4, H2)).
+        * intros v1' v2' Hin1 Hin2 Hyp.
+          assert (Hinv1 : val_loc v1' \subset dom H1).
+          { eapply Included_trans; [| now eapply in_dom_closed; eauto ].
+            eapply Included_trans; [| eassumption ].
+            simpl. rewrite post_Singleton; [| eassumption ].
+            eapply In_Union_list. eapply in_map. eassumption. }
+          assert (Hinv2 : val_loc v2' \subset dom H2).
+          { eapply Included_trans; [| now eapply in_dom_closed; eauto ].
+            eapply Included_trans; [| eassumption ].
+            simpl. rewrite post_Singleton; [| eassumption ].
+            eapply In_Union_list. eapply in_map. eassumption. }
+          rewrite res_approx_fuel_eq. eapply H; eauto.
+          rewrite <- res_approx_fuel_eq. eapply Hyp; eauto.
+          eapply Included_trans; [| now eapply closed_reach_in_S; eauto ].
+          eapply Included_trans; [| now eapply reach'_set_monotonic; eauto ].
+          eapply Included_trans; [| now eapply Included_post_reach'; eauto ].
+          eapply post_set_monotonic.
+          simpl. rewrite post_Singleton; [| eassumption ].
+          eapply In_Union_list. eapply in_map. eassumption.
+          eapply Included_trans; [| now eapply closed_reach_in_S; eauto ].
+          eapply Included_trans; [| now eapply reach'_set_monotonic; eauto ].
+          eapply Included_trans; [| now eapply Included_post_reach'; eauto ].
+          eapply post_set_monotonic.
+          simpl. rewrite post_Singleton; [| eassumption ].
+          eapply In_Union_list. eapply in_map. eassumption.
+        * eapply Forall2_monotonic; [| eauto ].
+          intros. eassumption.
+      - edestruct Heq as [rho2 [Hgetl2 Hall]]; eauto.
+        subst_exp.
+        eexists; split; [ now eauto |].
+        intros x.
+        edestruct Hall as [[v1 [v2 [Hs1 [Hs2 Hi]]]] | Hnone]; eauto.
+        left. repeat eexists; eauto. intros i' Hlt.
+        rewrite res_approx_fuel_eq. eapply H; eauto.
+        + rewrite <- res_approx_fuel_eq. eapply Hi. eassumption.
+        + eapply Included_trans; [| now eapply in_dom_closed; eauto ].
+          eapply Included_trans; [| eassumption ].
+          simpl. rewrite post_Singleton; [| eassumption ].
+          eapply get_In_env_locs. now constructor. eassumption. 
+        + eapply Included_trans; [| now eapply in_dom_closed; eauto ].
+          eapply Included_trans; [| eassumption ].
+          simpl. rewrite post_Singleton; [| eassumption ].
+          eapply get_In_env_locs. now constructor. eassumption.
+        + eapply Included_trans; [| now eapply closed_reach_in_S; eauto ].
+          eapply Included_trans; [| now eapply reach'_set_monotonic; eauto ].
+          eapply Included_trans; [| now eapply Included_post_reach'; eauto ].
+          eapply post_set_monotonic.
+          simpl. rewrite post_Singleton; [| eassumption ].
+          eapply get_In_env_locs. now constructor. eassumption.
+        + eapply Included_trans; [| now eapply closed_reach_in_S; eauto ].
+          eapply Included_trans; [| now eapply reach'_set_monotonic; eauto ].
+          eapply Included_trans; [| now eapply Included_post_reach'; eauto ].
+          eapply post_set_monotonic.
+          simpl. rewrite post_Singleton; [| eassumption ].
+          eapply get_In_env_locs. now constructor. eassumption. }
+    { simpl in *; eassumption. }
+  Qed.
+
+
+  Corollary res_equiv_weakening_alt (S1 S2 : Ensemble loc) (H1 H2 H1' H2' : heap block)
+            (v1 v2 : value) :
+    closed S1 H1 -> closed S2 H2 ->
+    (v1, H1) ≈ (v2, H2) ->
+    H1 ⊑ H1' ->
+    H2 ⊑ H2' ->
+    (val_loc v1) \subset dom H1 ->
+    (val_loc v2) \subset dom H2 ->
+    post H1 (val_loc v1) \subset S1 ->
+    post H2 (val_loc v2) \subset S2 ->
+    (v1, H1') ≈ (v2, H2').
+  Proof.
+    intros Hwf1 Hwf2 Heq Hsub1 Hsub2 Hp1 Hp2 Hin1 Hin2 n. destruct (Heq n) as [Heq1 He2].
+    split; rewrite res_approx_fuel_eq.
+    eapply (res_approx_weakening_alt S1 S2 H1 H2 H1' H2'); eauto.
+    now rewrite <- res_approx_fuel_eq.
+    eapply (res_approx_weakening_alt S2 S1 H2 H1 H2' H1'); eauto.
+    now rewrite <- res_approx_fuel_eq. 
+  Qed.
+
+  Lemma heap_env_approx_weakening_alt S S1 S2 H1 H2 H1' H2' rho1 rho2 :
+     closed S1 H1 -> closed S2 H2 ->
+     env_locs rho1 S \subset dom H1 ->
+     env_locs rho2 S \subset dom H2 ->
+     post H1 (env_locs rho1 S) \subset S1 ->
+     post H2 (env_locs rho2 S) \subset S2 ->
+     S |- (H1, rho1) ⩪ (H2, rho2) ->
+     H1 ⊑ H1' ->
+     H2 ⊑ H2' ->
+     heap_env_approx S (H1', rho1) (H2', rho2).
+  Proof.
+    intros Hwf1 Hwf2 He1 He2 Hp1 Hp2 [Heq1 Heq2] Hal1 Hal2 y l Hin Hget; simpl.
+    edestruct Heq1 as [x' [Hget' Heq']]; eauto.
+    eexists; split; eauto.
+    eapply (res_equiv_weakening_alt _ _ H1 H2); eauto.
+    eapply Included_trans; [| eassumption ].
+    now eapply get_In_env_locs; eauto.
+    eapply Included_trans; [| eassumption ].
+    now eapply get_In_env_locs; eauto.
+    eapply Included_trans; [| eassumption ].
+    eapply post_set_monotonic.
+    now eapply get_In_env_locs; eauto.
+    eapply Included_trans; [| eassumption ].
+    eapply post_set_monotonic.
+    now eapply get_In_env_locs; eauto.
+  Qed.
+  
+  Corollary heap_env_equiv_weaking_alt S S1 S2 H1 H2 H1' H2' rho1 rho2 :
+    closed S1 H1 -> closed S2 H2 ->
+    env_locs rho1 S \subset dom H1 ->
+    env_locs rho2 S \subset dom H2 ->
+    post H1 (env_locs rho1 S) \subset S1 ->
+    post H2 (env_locs rho2 S) \subset S2 ->
+    S |- (H1, rho1) ⩪ (H2, rho2) ->
+    H1 ⊑ H1' ->
+    H2 ⊑ H2' ->
+    S |- (H1', rho1) ⩪ (H2', rho2).
+  Proof.
+    intros. split.
+    now eapply (heap_env_approx_weakening_alt _ _ _ H1 H2); eauto.
+    now eapply (heap_env_approx_weakening_alt _ _ _ H2 H1); eauto; symmetry.
+  Qed.
+  
+  (** Preservation under store and heap extension *)
+  
+  Lemma heap_env_approx_set S H1 H2 x l1 l2 rho1 rho2 :
+    heap_env_approx (Setminus _ S (Singleton _ x)) (H1, rho1) (H2, rho2) ->
+    (l1, H1) ≈ (l2, H2) ->
+    heap_env_approx S (H1, M.set x l1 rho1) (H2, M.set x l2 rho2).
+  Proof.
+    intros Heq Hreq. intros y l Hin Hget.
+    destruct (peq x y); subst; simpl in *. 
+    - exists l2. rewrite M.gss in *; inv Hget; eauto.
+        - rewrite M.gso in *; eauto. eapply Heq in Hget; eauto.
+          constructor; eauto. intros Hc; inv Hc; congruence.
+  Qed.
+
+  Lemma heap_env_equiv_set S H1 H2 x l1 l2 rho1 rho2 :
+    Setminus _ S (Singleton _ x) |- (H1, rho1) ⩪ (H2, rho2) ->
+    (l1, H1) ≈ (l2, H2) ->
+    S  |- (H1, M.set x l1 rho1) ⩪ (H2, M.set x l2 rho2).
+  Proof.
+    intros [Heq1 Heq2] Hreq. split.
+    now eapply heap_env_approx_set.
+    now eapply heap_env_approx_set; eauto; symmetry.
+  Qed.
+
+    Lemma heap_env_approx_alloc S S1 S2 H1 H2 H1' H2' rho1 rho2 l1 l2 b1 b2 x :
+    closed S1 H1 -> closed S2 H2 ->
+    env_locs rho1 (S \\ [set x]) \subset S1 ->
+    env_locs rho2 (S \\ [set x]) \subset S2 ->
+    locs b1 \subset S1 -> locs b2 \subset S2 ->
+    S \\ [set x] |- (H1, rho1) ⩪ (H2, rho2) ->
+    alloc b1 H1 = (l1, H1') -> 
+    alloc b2 H2 = (l2, H2') ->
+    block_equiv (H1, b1) (H2, b2) ->
+    heap_env_approx S (H1', M.set x (Loc l1) rho1) (H2', M.set x (Loc l2) rho2).
+  Proof.
+    intros Hc1 Hc2 Hsub1 Hsub2 Hin1 Hin2 Heq Ha1 Ha2 Hb y v1 Hin Hget.
+    destruct (peq x y); subst.
+    - rewrite M.gss in Hget. inv Hget.
+      eexists; split. rewrite M.gss. reflexivity.
+      rewrite res_equiv_eq. simpl.
+      erewrite gas; eauto. erewrite gas; eauto.
+      simpl in Hb. destruct b1; destruct b2; try contradiction.
+      + destruct Hb as [Heq' Hall]; subst.
+        split; eauto.
+        eapply Forall2_monotonic_strong; eauto.
+        intros. 
+        eapply res_equiv_weakening. exact Hc1. exact Hc2.
+        eassumption.
+        now eapply alloc_subheap; eauto.
+        now eapply alloc_subheap; eauto.
+        eapply Included_trans; [| eassumption ].
+        eapply In_Union_list. now eapply in_map; eauto.
+        eapply Included_trans; [| eassumption ].
+        eapply In_Union_list. now eapply in_map; eauto.
+      + eapply heap_env_equiv_weaking'.
+        exact Hc1. exact Hc2.
+        eassumption. eassumption. eassumption.
+        now eapply alloc_subheap; eauto.
+        now eapply alloc_subheap; eauto.
+    - rewrite M.gso in Hget; eauto.
+      destruct Heq as [Heq1 Heq2].
+      edestruct Heq1 as [v2 [Hget2 Hb']]; eauto.
+      constructor; eauto. now intros Hc; inv Hc; eauto.
+      eexists.
+      rewrite M.gso; eauto. split; eauto.
+      eapply res_equiv_weakening. exact Hc1. exact Hc2.
+      eassumption.
+      now eapply alloc_subheap; eauto.
+      now eapply alloc_subheap; eauto.
+      eapply Included_trans; [| now apply Hsub1 ].
+      eapply get_In_env_locs; eauto.
+      constructor; eauto. now intros Hc; inv Hc; eauto.
+      eapply Included_trans; [| now apply Hsub2 ].
+      eapply get_In_env_locs; eauto.
+      constructor; eauto. now intros Hc; inv Hc; eauto.      
+  Qed.
+  
+  Corollary heap_env_equiv_alloc S S1 S2 H1 H2 H1' H2' rho1 rho2 l1 l2 b1 b2 x :
+    closed S1 H1 -> closed S2 H2 ->
+    env_locs rho1 (S \\ [set x]) \subset S1 ->
+    env_locs rho2 (S \\ [set x]) \subset S2 ->
+    locs b1 \subset S1 -> locs b2 \subset S2 ->
+    S \\ [set x] |- (H1, rho1) ⩪ (H2, rho2) ->
+    alloc b1 H1 = (l1, H1') -> 
+    alloc b2 H2 = (l2, H2') ->
+    block_equiv (H1, b1) (H2, b2) ->
+    S |- (H1', M.set x (Loc l1) rho1) ⩪ (H2', M.set x (Loc l2) rho2).
+  Proof.
+    intros. split. now eapply (heap_env_approx_alloc S S1 S2); eauto.
+    eapply (heap_env_approx_alloc S S2 S1); eauto; symmetry; eassumption.
+  Qed.
+
+  Lemma heap_env_approx_alloc_alt S S1 S2 H1 H2 H1' H2' rho1 rho2 l1 l2 b1 b2 x :
+    closed S1 H1 -> closed S2 H2 ->
+    env_locs rho1 (S \\ [set x]) \subset S1 ->
+    env_locs rho2 (S \\ [set x]) \subset S2 ->
+    locs b1 \subset dom H1 ->
+    locs b2 \subset dom H2 ->
+    post H1 (locs b1) \subset S1 ->
+    post H2 (locs b2) \subset S2 ->
+    S \\ [set x] |- (H1, rho1) ⩪ (H2, rho2) ->
+    alloc b1 H1 = (l1, H1') -> 
+    alloc b2 H2 = (l2, H2') ->
+    block_equiv (H1, b1) (H2, b2) ->
+    heap_env_approx S (H1', M.set x (Loc l1) rho1) (H2', M.set x (Loc l2) rho2).
+  Proof.
+    intros Hc1 Hc2 Hsub1 Hsub2 Hl1 Hl2 Hp1 Hp2 Heq Ha1 Ha2 Hb y v1 Hin Hget.
+    destruct (peq x y); subst.
+    - rewrite M.gss in Hget. inv Hget.
+      eexists; split. rewrite M.gss. reflexivity.
+      rewrite res_equiv_eq. simpl.
+      erewrite gas; eauto. erewrite gas; eauto.
+      simpl in Hb. destruct b1; destruct b2; try contradiction.
+      + destruct Hb as [Heq' Hall]; subst.
+        split; eauto.
+        eapply Forall2_monotonic_strong; eauto.
+        intros. 
+        eapply res_equiv_weakening_alt.
+        * exact Hc1.
+        * exact Hc2.
+        * eassumption.
+        * now eapply alloc_subheap; eauto.
+        * now eapply alloc_subheap; eauto.
+        * eapply Included_trans; [| eassumption ].
+          eapply In_Union_list. eapply in_map. eassumption.
+        * eapply Included_trans; [| eassumption ].
+          eapply In_Union_list. eapply in_map. eassumption.
+        * eapply Included_trans; [| eassumption ].
+          eapply post_set_monotonic.
+          eapply In_Union_list. eapply in_map. eassumption.
+        * eapply Included_trans; [| eassumption ].
+          eapply post_set_monotonic.
+          eapply In_Union_list. eapply in_map. eassumption.
+      + simpl in *.
+        eapply heap_env_equiv_weaking_alt; [ exact Hc1 | exact Hc2 | | | | | | |]; try eassumption.
+        now eapply alloc_subheap; eauto.
+        now eapply alloc_subheap; eauto.
+    - rewrite M.gso in Hget; eauto.
+      destruct Heq as [Heq1 Heq2].
+      edestruct Heq1 as [v2 [Hget2 Hb']]; eauto.
+      constructor; eauto. now intros Hc; inv Hc; eauto.
+      eexists.
+      rewrite M.gso; eauto. split; eauto.
+      eapply res_equiv_weakening_alt.
+      + exact Hc1.
+      + exact Hc2.
+      + eassumption.
+      + now eapply alloc_subheap; eauto.
+      + now eapply alloc_subheap; eauto.
+      + eapply Included_trans; [| now eapply in_dom_closed; eauto ].
+        eapply Included_trans; [| now apply Hsub1 ].
+        eapply get_In_env_locs; [| eassumption ].
+        constructor; eauto. now intros Hc; inv Hc; eauto.
+      + eapply Included_trans; [| now eapply in_dom_closed; eauto ].
+        eapply Included_trans; [| now apply Hsub2 ].
+        eapply get_In_env_locs; [| eassumption ].
+        constructor; eauto. now intros Hc; inv Hc; eauto.
+      + eapply Included_trans; [| now eapply closed_reach_in_S; eauto ].
+        eapply Included_trans; [| now eapply Included_post_reach'; eauto ].
+        eapply post_set_monotonic.
+        eapply Included_trans; [| now apply Hsub1 ].
+        eapply get_In_env_locs; [| eassumption ].
+        constructor; eauto. now intros Hc; inv Hc; eauto.
+      + eapply Included_trans; [| now eapply closed_reach_in_S; eauto ].
+        eapply Included_trans; [| now eapply Included_post_reach'; eauto ].
+        eapply post_set_monotonic.
+        eapply Included_trans; [| now apply Hsub2 ].
+        eapply get_In_env_locs; [| eassumption ].
+        constructor; eauto. now intros Hc; inv Hc; eauto.
+  Qed.
+
+  Corollary heap_env_equiv_alloc_alt S S1 S2 H1 H2 H1' H2' rho1 rho2 l1 l2 b1 b2 x :
+    closed S1 H1 -> closed S2 H2 ->
+    env_locs rho1 (S \\ [set x]) \subset S1 ->
+    env_locs rho2 (S \\ [set x]) \subset S2 ->
+    locs b1 \subset dom H1 ->
+    locs b2 \subset dom H2 ->
+    post H1 (locs b1) \subset S1 ->
+    post H2 (locs b2) \subset S2 ->
+    S \\ [set x] |- (H1, rho1) ⩪ (H2, rho2) ->
+    alloc b1 H1 = (l1, H1') -> 
+    alloc b2 H2 = (l2, H2') ->
+    block_equiv (H1, b1) (H2, b2) ->
+    S |- (H1', M.set x (Loc l1) rho1) ⩪ (H2', M.set x (Loc l2) rho2).
+  Proof.
+    intros. split. now eapply (heap_env_approx_alloc_alt S S1 S2); eauto.
+    eapply (heap_env_approx_alloc_alt S S2 S1); eauto; symmetry; eassumption.
+  Qed.
+
+  Lemma heap_env_equiv_setlist S H1 H2 xs ls1 ls2 rho1 rho2 rho1' rho2' :
+    Setminus _ S (FromList xs) |- (H1, rho1) ⩪ (H2, rho2) ->
+    setlist xs ls1 rho1 = Some rho1' -> setlist xs ls2 rho2 = Some rho2' ->
+    Forall2 (fun l1 l2 => (l1, H1) ≈ (l2, H2)) ls1 ls2  ->
+    S |- (H1, rho1') ⩪ (H2, rho2').
+  Proof with (now eauto with Ensembles_DB).
+    revert S rho1' rho2' ls1 ls2; induction xs;
+    intros S  rho1' rho2' ls1 ls2 Heq Hs1 Hs2 Hall.
+    - destruct ls1; destruct ls2; try discriminate. inv Hs1; inv Hs2; eauto.
+      rewrite FromList_nil, Setminus_Empty_set_neut_r in Heq. eassumption.
+    - destruct ls1; destruct ls2; try discriminate.
+      inv Hall. simpl in Hs1, Hs2.
+      destruct (setlist xs ls1 rho1) eqn:Hset1; try discriminate.
+      destruct (setlist xs ls2 rho2) eqn:Hset2; try discriminate.
+      inv Hs1; inv Hs2. eapply heap_env_equiv_set; eauto.
+      eapply IHxs; eauto. eapply heap_env_equiv_antimon; eauto.
+      rewrite FromList_cons...
+  Qed.
+
+  Lemma heap_env_equiv_def_funs S S1 S2 H1 H2 rho1 rho2 clo_rho1 clo_rho2 B B0 c l1 l2 :
+    closed S1 H1 -> closed S2 H2 ->
+    env_locs rho1 (Setminus _ S (name_in_fundefs B)) \subset S1 ->
+    env_locs rho2 (Setminus _ S (name_in_fundefs B)) \subset S2 ->
+    get l1 H1 = Some (Env clo_rho1) ->
+    get l2 H2 = Some (Env clo_rho2) ->
+    env_locs clo_rho1 (Full_set _) \subset S1 ->
+    env_locs clo_rho2 (Full_set _) \subset S2 ->
+    (occurs_free_fundefs B0) \subset (Setminus _ S (name_in_fundefs B)) ->
+    (Loc l1, H1) ≈ (Loc l2, H2) ->             
+    Setminus _ S (name_in_fundefs B) |- (H1, rho1) ⩪ (H2, rho2) ->
+    S |- (def_closures B B0 rho1 H1 c l1) ⩪ (def_closures B B0 rho2 H2 c l2).
+  Proof with (now eauto with Ensembles_DB).
+    revert S rho1 rho2; induction B;
+    intros S rho1 rho2 Hc1 Hc2 Hinl1 Hinl2 He1 He2 Hg1 Hg2 Hsub Hloc Heq; simpl; eauto.
+    - destruct (def_closures B B0 rho1 H1 c l1) as [H1' rho1'] eqn:Hd1.
+      destruct (def_closures B B0 rho2 H2 c l2) as [H2' rho2'] eqn:Hd2.
+      destruct (alloc (Constr c [FunPtr B0 v; Loc l1]) _) as [l1' H1''] eqn:Ha1.
+      destruct (alloc (Constr c [FunPtr B0 v; Loc l2]) _) as [l2' H2''] eqn:Ha2.
+      edestruct (def_funs_exists_new_set (S \\ [set v]) S1 H1 H1' rho1 rho1' clo_rho1 B) as [S1' [HsubS1 [Hcl1 Henv1]]]; eauto.
+      eapply Included_trans; [| now apply Hinl1 ]. simpl. rewrite <- !Setminus_Union...
+      edestruct (def_funs_exists_new_set (S \\ [set v]) S2 H2 H2' rho2 rho2' clo_rho2 B) as [S2' [HsubS2 [Hcl2 Henv2]]]; eauto.
+      eapply Included_trans; [| now apply Hinl2 ]. simpl. rewrite <- !Setminus_Union...
+      eapply heap_env_equiv_alloc_alt; (try now apply Ha1); (try now apply Ha2); eauto.
+      + simpl. rewrite Union_Empty_set_neut_r, Union_Empty_set_neut_l.
+        eapply Singleton_Included. eapply dom_subheap.
+        eapply def_funs_subheap. now eauto. now eexists; eauto.
+      + simpl. rewrite Union_Empty_set_neut_r, Union_Empty_set_neut_l.
+        eapply Singleton_Included. eapply dom_subheap.
+        eapply def_funs_subheap. now eauto. now eexists; eauto.
+      + simpl. rewrite Union_Empty_set_neut_r, Union_Empty_set_neut_l.
+        rewrite post_Singleton; [| eapply def_funs_subheap; now eauto ].
+        eapply Included_trans...
+      + simpl. rewrite Union_Empty_set_neut_r, Union_Empty_set_neut_l.
+        rewrite post_Singleton; [| eapply def_funs_subheap; now eauto ].
+        eapply Included_trans...
+      + setoid_rewrite <- Hd1. setoid_rewrite <- Hd2.
+        simpl in Heq, Hinl1, Hinl2. rewrite <- !Setminus_Union in Heq, Hinl1, Hinl2.
+        eapply IHB; try eassumption.
+        eapply Included_trans; [ eassumption |]. simpl. rewrite <- !Setminus_Union...
+      + simpl. split. now eauto.
+        constructor.
+        * rewrite res_equiv_eq. simpl; split; eauto.
+        *  constructor. eapply res_equiv_weakening_alt.
+           now apply Hc1. now apply Hc2. eassumption.
+           now eapply def_funs_subheap; eauto.
+           now eapply def_funs_subheap; eauto.
+           eapply Singleton_Included. now eexists; eauto.
+           eapply Singleton_Included. now eexists; eauto.
+           simpl. rewrite post_Singleton; [ | eassumption ].
+           eassumption. 
+           simpl. rewrite post_Singleton; [ | eassumption ].
+           eassumption. 
+           now constructor.
+    - simpl. rewrite Setminus_Empty_set_neut_r in Heq.
+      eassumption.
+  Qed.
+
+  
+  Lemma res_equiv_get_Constr (H1 H2 : heap block)
+        (l1 l2 : loc) (c : cTag) (vs1 : list value) :
+    (Loc l1, H1) ≈ (Loc l2, H2) ->
+    get l1 H1 = Some (Constr c vs1) ->
+    exists vs2,
+      get l2 H2 = Some (Constr c vs2) /\
+      Forall2 (fun v1 v2 => (v1, H1) ≈ (v2, H2)) vs1 vs2.
+  Proof.
+    intros Hres Hget. 
+    rewrite res_equiv_eq in Hres. simpl in Hres. rewrite Hget in Hres.
+    destruct (get l2 H2); try contradiction.
+    destruct b; try contradiction. 
+    destruct Hres as [Heq Hb]. subst. eexists; split; eauto. 
+  Qed.
+
+  Lemma heap_env_equiv_env_get (S : Ensemble var) (H1 H2 : heap block)
+        (rho1 rho2 : env) (x : var) (l : value) :
+    M.get x rho1 = Some l ->
+    S |- (H1, rho1) ⩪ (H2, rho2) ->
+    x \in S ->
+    exists l',
+      M.get x rho2 = Some l' /\
+      (l, H1) ≈ (l', H2).
+  Proof.
+    intros Hget Heq Hin.
+    eapply Heq in Hget; eassumption.
+  Qed.
+  
+  Lemma heap_env_equiv_env_getlist (S : Ensemble var) (H1 H2 : heap block)
+        (rho1 rho2 : env) (xs : list var) (ls : list value) :
+    getlist xs rho1 = Some ls ->
+    S |- (H1, rho1) ⩪ (H2, rho2) ->
+    (FromList xs) \subset S ->
+    exists ls',
+      getlist xs rho2 = Some ls' /\
+      Forall2 (fun l l' => (l, H1) ≈ (l', H2)) ls ls'.
+  Proof with now eauto with Ensembles_DB.
+    revert ls; induction xs; intros ls Hget Heq Hin.
+    - inv Hget.
+      eexists; split; eauto. reflexivity.
+    - simpl in Hget.
+      destruct (M.get a rho1) as [l1 | ] eqn:Hgetl1; try discriminate.
+      destruct (getlist xs rho1) as [ls1 | ] eqn:Hetls1; try discriminate.
+      inv Hget.
+      edestruct heap_env_equiv_env_get as [l2 [Hgetl2 Heq']]; eauto.
+      eapply Hin. rewrite FromList_cons...
+      edestruct IHxs as [ls2 [Hgetls2 Hall2]]; eauto.
+      eapply Included_trans; try eassumption. 
+      rewrite FromList_cons...
+      eexists; split. simpl. rewrite Hgetl2, Hgetls2.
+      reflexivity. constructor; eauto.
+  Qed.
+
+
+  Lemma heap_env_equiv_getlist_Forall2 S H1 H2 ys vs1 vs2 rho1 rho2 :
+    S |- (H1, rho1) ⩪ (H2, rho2) ->
+    FromList ys \subset S ->
+    getlist ys rho1 = Some vs1 ->
+    getlist ys rho2 = Some vs2 ->
+    Forall2 (fun l1 l2 => (l1, H1) ≈ (l2, H2)) vs1 vs2.
+  Proof.
+    revert vs1 vs2; induction ys; intros vs1 vs2 Heq Hin Hg1 Hg2;
+    destruct vs1; destruct vs2; simpl in *; try discriminate; try now constructor.
+    - destruct (M.get a rho1) eqn:Heqa;
+      destruct (getlist ys rho1) eqn:Heqys; try discriminate.
+    - destruct (M.get a rho2) eqn:Heqa;
+      destruct (getlist ys rho2) eqn:Heqys; try discriminate.
+    - rewrite FromList_cons in Hin.
+      destruct (M.get a rho1) eqn:Heqa;
+        destruct (getlist ys rho1) eqn:Heqys; try discriminate. inv Hg1.
+      eapply Heq in Heqa. destruct Heqa as [l' [Hget Heq']].
+      rewrite Hget in Hg2.
+      destruct (getlist ys rho2) eqn:Heqys'; try discriminate. inv Hg2.
+      constructor; eauto. eapply IHys; eauto.
+      eapply Included_trans; now eauto with Ensembles_DB.
+      eapply Included_trans; now eauto with Ensembles_DB.
+  Qed.
+
+  Lemma block_equiv_Constr (H1 H2 : heap block) (c : cTag) (vs vs' : list value) :
+    Forall2 (fun l1 l2 => (l1, H1) ≈ (l2, H2)) vs vs' ->
+    block_equiv (H1, Constr c vs) (H2, Constr c vs').
+  Proof.
+    simpl; split; eauto.
+  Qed.
+
+  Lemma block_equiv_Fun (H1 H2 : heap block) (rho1 rho2 : env) :
+    Full_set _ |- (H1, rho1) ⩪ (H2, rho2) ->
+    block_equiv (H1, Env rho1) (H2, Env rho2).
+  Proof.
+    simpl; eauto.
+  Qed.
+  
+  (** * Lemmas about [live] *)  
+
+  Lemma live_exists S H :
+    Decidable S ->
+    exists H', live S H H'.
+  Proof.
+  Admitted.
+  
+  Lemma live_deterministic S H1 H2 H2' :
+    live S H1 H2 ->
+    live S H1 H2' ->
+    S |- H2 ≃ H2'.
+  Proof.
+    intros [Hyp1 [Hyp2 Hyp3]] [Hyp1' [Hyp2' Hyp3']].
+    eapply Equivalence.equiv_transitive; eauto.
+    symmetry. eassumption.
+  Qed.
+
+  Lemma live_collect S H1 H2 :
+    live S H1 H2 ->
+    collect S H1 H2.
+  Proof.
+    firstorder.
+  Qed.
+  
+  Lemma live_idempotent (S : Ensemble loc) (H1 H2 : heap block) :
+    live S H1 H2 ->
+    live S H2 H2.
+  Proof.
+    intros Hl.
+    assert (Hc := live_collect _ _ _ Hl).
+    destruct Hl as [Hyp1 [Hyp2 Hyp3]]. split; eauto.
+    split; eauto.
+    reflexivity. 
+  Qed.
+
+  Instance Properlive : Proper (Same_set _ ==> eq ==> eq ==> iff) live.
+  Proof.
+    constructor; subst; intros [Hl1 [Hl2 Hl3]].
+    split; eauto. split; eauto; now rewrite <- H.
+    split; eauto. split; eauto; now rewrite H.
+  Qed.
+
+
+  Lemma val_loc_in_dom (H1 H2 : heap block) (v1 v2 : value) :
+    (v1, H1) ≈ (v2, H2) ->
+    val_loc v1 \subset dom H1 ->
+    val_loc v2 \subset dom H2.
+  Proof.
+    intros Heq Hin.
+    rewrite res_equiv_eq in Heq.
+    destruct v1; destruct v2; try contradiction.
+    - destruct (Hin l) as [b Hb].
+      reflexivity. simpl in Heq. rewrite Hb in Heq. 
+      eapply Singleton_Included.
+      destruct b.
+      + destruct (get l0 H2) eqn:Heq'; try contradiction. 
+        now eexists; eauto.
+      + destruct (get l0 H2) eqn:Heq'; try contradiction. 
+        now eexists; eauto.
+    - simpl; now eauto with Ensembles_DB. 
+  Qed.
+
+  Lemma env_locs_in_dom S (H1 H2 : heap block) (rho1 rho2 : env) :
+    S |- (H1, rho1) ⩪ (H2, rho2) ->
+    env_locs rho1 S \subset dom H1 ->
+    env_locs rho2 S \subset dom H2.
+  Proof.
+    intros Heq Hsub l [y [Hin Hget]].
+    destruct (M.get y rho2) as [v |] eqn:Hget1; try now inv Hget.
+    edestruct Heq as [_ [v' [Hget2 Heqv]]]; eauto. 
+    symmetry in Heqv. eapply val_loc_in_dom; eauto.
+    eapply Included_trans; [| eassumption ].
+    eapply get_In_env_locs; eauto.
+  Qed.     
+
+  Lemma locs_in_dom (H1 H2 : heap block) (b1 b2 : block) :
+    block_equiv (H1, b1) (H2, b2) ->
+    locs b1 \subset dom H1 ->
+    locs b2 \subset dom H2.
+  Proof.
+    intros Hb Hin.
+    destruct b1; destruct b2; try contradiction.
+    - simpl in *. destruct Hb as [Heq Hall]; subst.
+      (* yikes. maybe write lemma? *)
+      induction Hall; try now eauto with Ensembles_DB.
+      simpl in *. eapply Union_Included.
+       eapply val_loc_in_dom; eauto.
+       now eapply Union_Included_l; eauto. 
+       eapply IHHall. now eapply Union_Included_r; eauto.
+     - simpl in *. eapply env_locs_in_dom; eauto.
+  Qed.
+
+  Lemma res_equiv_exists_loc H1 H2 v1 v2 l1 :
+    (v1, H1) ≈ (v2, H2) ->
+    l1 \in val_loc v1 ->
+    exists l2, l2 \in val_loc v2 /\ (Loc l1, H1) ≈ (Loc l2, H2).
+  Proof.
+    intros Heq Hin. rewrite res_equiv_eq in Heq.
+    destruct v1; destruct v2; try contradiction; inv Hin.
+    eexists; split. reflexivity. rewrite res_equiv_eq.
+    eassumption.
+  Qed.
+
+  Lemma heap_env_equiv_exists_loc S H1 H2 rho1 rho2 l1 :
+    S |- (H1, rho1) ⩪ (H2, rho2) ->
+    l1 \in env_locs rho1 S ->
+    exists l2, l2 \in env_locs rho2 S /\ (Loc l1, H1) ≈ (Loc l2, H2).
+  Proof.
+    intros Heq Hin. edestruct Hin as [x [Hin' Hget]].
+    destruct (M.get x rho1) as [v1 |] eqn:Hget1; [| now inv Hget].
+    edestruct Heq as [[v2 [Hget2 Heq']] _]; eauto.
+    destruct v1; [| now inv Hget].
+    destruct v2; [| rewrite res_equiv_eq in Heq'; contradiction ].
+    inv Hget. eexists; split; eauto.
+    eapply get_In_env_locs; eauto. reflexivity.
+  Qed.
+
+  Lemma block_equiv_exists_loc H1 H2 b1 b2 l1 :
+    block_equiv (H1, b1) (H2, b2) ->
+    l1 \in locs b1 ->
+    exists l2, l2 \in locs b2 /\ (Loc l1, H1) ≈ (Loc l2, H2).
+  Proof.
+    intros Hb Hin.
+    destruct b1; destruct b2; try contradiction; simpl in Hin.
+    - destruct Hb as [Heq Hall]. subst. 
+      induction Hall. now inv Hin.
+      simpl in Hin.
+      inv Hin.
+      + edestruct res_equiv_exists_loc as [l2 [Hl2in Heq]]; eauto.
+        eexists. split; eauto. left. eassumption.
+      + edestruct IHHall as [l2 [Hl2in Heq]]; eauto.
+        eexists. split; eauto. right. eassumption.
+    - eapply heap_env_equiv_exists_loc; eauto.
+  Qed.
+
+  Lemma heap_equiv_post S H1 H2 l1 n b1 :
+    S |- H1 ≃ H2 ->
+    In _ ((post H1 ^ n) S) l1 ->
+    get l1 H1 = Some b1 ->
+    exists l2 b2, In _ ((post H2 ^ n) S) l2 /\ get l2 H2 = Some b2 /\
+             block_equiv (H1, b1) (H2, b2).
+  Proof.
+    intros Heq.
+    revert l1 b1. induction n as [| n IHn]; intros l1 b1 Hin Hget.
+    - edestruct Heq as [[le Heq'] _]; eauto.
+    - simpl in Hin. simpl.
+      destruct Hin as [l1' [b1' [Hin [Hget' Hin']]]]. 
+      edestruct IHn as [l2' [b2' [Hpost [Hget2 Heqb]]]]; eauto.
+      simpl in Heqb.
+      edestruct block_equiv_exists_loc as [l2 [Hl2in Hleq]]; eauto.
+      rewrite res_equiv_eq in Hleq. simpl in Hleq. rewrite Hget in Hleq.
+      destruct (get l2 H2) as [b2 |] eqn:Hgetl2; try contradiction.
+      exists l2, b2. split; [| split; now eauto ].
+      eexists. eexists. split; eauto.
+  Qed.
+
+
+  Lemma heap_equiv_respects_well_formed S H1 H2 :
+    S |- H1 ≃ H2 ->
+    well_formed (reach' H1 S) H1 ->
+    well_formed (reach' H2 S) H2.
+  Proof.
+    intros Heq Hwf l2 b2 [n [_ Hin]] Heq2.
+    symmetry in Heq. 
+    edestruct heap_equiv_post as [l1 [b1 [Hpost1 [Hget1 Heq1]]]]; eauto.
+    eapply Hwf in Hget1; [| eexists; split; [ now constructor | now eauto ]].
+    eapply locs_in_dom; eauto. symmetry; eassumption.
+  Qed.
+  
+  Lemma heap_equiv_in_dom S S' H1 H2 :
+    S |- H1 ≃ H2 ->
+    S' \subset S ->
+    S' \subset dom H1 ->
+    S' \subset dom H2.
+  Proof.
+    intros Heq Hsub Hsub1 l Hin.
+    edestruct Hsub1 as [b Hget]; eauto.
+    edestruct Heq as [[b' [Hget' _]] _]; eauto.
+    eexists; eauto.
+  Qed.
+  
+  Lemma heap_env_approx_restrict_env S S' H1 H2 rho1 rho1' rho2 rho2' :
+    heap_env_approx S (H1, rho1) (H2, rho2) ->
+    S' \subset S ->
+    restrict_env S' rho1 rho1' ->
+    restrict_env S' rho2 rho2' ->
+    heap_env_approx (Full_set _) (H1, rho1') (H2, rho2').
+  Proof. 
+    intros Ha Hsub [Heq1 [Hsub1 Hk1]] [Heq2 [Hsub2 Hk2]] x l Hin Hget.
+    edestruct Ha as [l' [Hget' Heq]].
+    eapply Hsub. eapply Hk1. unfold key_set, In. now rewrite Hget; eauto.
+    eapply Hsub1. eassumption.
+    eexists. split; eauto.
+    rewrite <- Heq2. eassumption. eapply Hk1.
+    unfold key_set, In. now rewrite Hget; eauto.
+  Qed.
+
+  Corollary heap_env_equiv_restrict_env S S' H1 H2 rho1 rho1' rho2 rho2' :
+    S |- (H1, rho1) ⩪ (H2, rho2) ->
+    S' \subset S ->
+    restrict_env S' rho1 rho1' ->
+    restrict_env S' rho2 rho2' ->
+    Full_set var |- (H1, rho1') ⩪ (H2, rho2').
+  Proof.
+    intros [? ?] ? ? ?.
+    split; now eapply heap_env_approx_restrict_env; eauto.
+  Qed.
+
+End HeapEquiv. 
